\documentclass[12pt]{article}
\usepackage[margin=1in]{geometry} 
\usepackage{amsmath,amsthm,amssymb,amsfonts}
 
\newcommand{\N}{\mathbb{N}}
\newcommand{\Z}{\mathbb{Z}}
 
\newenvironment{problem}[2][Problem]{\begin{trivlist}
\item[\hskip \labelsep {\bfseries #1}\hskip \labelsep {\bfseries #2.}]}{\end{trivlist}}
 
\begin{document}

\title{MA1101R Linear Algebra Tutorial 4}
\author{Lim Wen Bin}
\maketitle
 


\begin{problem}{1.a.i}
\end{problem}
\begin{align*}
\det(A) &= 
	\left| 
	\begin{array}{ccc}
	0 & 1 & -1\\
	1 & 0 & -2\\
	1 & -1 & 0 
	\end{array} 
	\right| \\
&= - \left| 
	\begin{array}{cc}
	1 & -2\\
	1 & 0 
	\end{array} 
	\right| -
	\left| 
	\begin{array}{cc}
	1 & 0 \\
	1 & -1
	\end{array} 
	\right| \\
&=  -2 + 1 \\
&= -1
\end{align*}

\begin{problem}{2}
\end{problem}
\begin{proof}
\begin{align*} 
\intertext{Let matrix be A. Let B be the matrix obtained from adding the $m$ rows of the given matrix multiplied by $10^{6-m}$ to the first row.}
\det(B) = 10000 \times 1000 \times 100 \times 10 \times \det(A) \\
\intertext{By cofactor expansion,}
\det(B) = 11322 B_{1,1} + 13209 B_{1,2} + 29189 B_{1,3} + 56661 B_{1,4} + 15096 B_{1,5} \\
17 \not | 10000 \times 1000 \times 100 \times 10 \land 17 | \det(B) \Rightarrow 17 | \det(A)
\end{align*}
\end{proof}

\begin{problem}{3.c}
\end{problem}
\begin{align*} 
\det(A) = \det(B) &\not \Rightarrow A = B \\
\therefore \det(A+C) &\ne \det(B+C)
\end{align*}

\begin{problem}{3.d}
\end{problem}
\begin{align*} 
\det(AB) &= \det(A) \det(B) \\
&= \det(B) \det(A) & (\text{$\because$ multiplication is commutative for real numbers})\\ 
&= \det(BA)
\end{align*}

\begin{problem}{3.e}
\end{problem}
\begin{align*} 
\text{In general, } AB &\ne BA \\
\therefore \det(A+C) &\ne \det(B+C)
\end{align*}

\begin{problem}{3.e}
\end{problem}
\begin{align*}
A &= PBP^{-1}\\ 
\det(A) &= \det(P) \det(B) \det(P^{-1})\\
&= \det(P) \det(B) \frac{1}{\det(P)}\\
&= \det(B)\\
\end{align*}

\begin{problem}{3.e}
\end{problem}
\begin{align*}
\intertext{For $n\times n$ $A$,}
\det(cA) = c^n \det(A) & (\text{$\because cA$ is obtained from multiplying every row of $A$ by $c$})
\end{align*}

\begin{problem}{4.a}
\end{problem}
\begin{proof}
\begin{align*}
A^{-1} &= \frac{1}{\det(A)}\operatorname{adj}(A)\\
I &= \frac{1}{\det(A)} A \operatorname{adj}(A)\\
\therefore \text{A is invertible and } \operatorname{adj}(A)^{-1} &= \frac{1}{\det(A)} A 
\end{align*}
\end{proof}

\begin{problem}{4.b}
\end{problem}
\begin{align*}
A^{-1} &= \frac{1}{\det(A)}\operatorname{adj}(A)\\
\operatorname{adj}(A) &= \det(A) A^{-1}\\
\det(\operatorname{adj}(A)) &= \det(\det(A) A^{-1})\\
&= \det(A)^n \det(A^{-1})\\
&= \det(A)^{n-1}
\end{align*}

\begin{problem}{4.b}
\end{problem}
\begin{proof}
\begin{align*}
\det(A) &= 1\\
\operatorname{adj}(A) &= \det(A) A^{-1}\\
& = A^{-1}\\
\operatorname{adj}(\operatorname{adj}(A)) &= \det(\operatorname{adj}(A)) (\operatorname{adj}(A))^{-1}\\
&= \det(A^{-1}) (A^{-1})^{-1}\\
&= \frac{1}{\det(A)} A\\
&= A
\end{align*}
\end{proof}

\begin{problem}{5.a}
\end{problem}
\begin{align*}
y - 2 &= -3(x-1)\\
y + 3x &= 5\\
\text{Implicit form: } &\{ (x,y) | y + 3x = -1 \}\\
\text{Explicit form: } &\{ (t, 5-3t | t \in \mathbb{R} \}\\
\end{align*}

\begin{problem}{5.b}
\end{problem}
\begin{align*}
\vec u &= \left( \begin{array}{c}
	1 \\ -2 \\ 1
	\end{array}
	\right)\\
\vec v &= \left( \begin{array}{c}
	-1 \\ 3 \\ 0
	\end{array}
	\right)\\
\vec n &= \vec u \times \vec v \\
&= \left( \begin{array}{c}
	-3 \\ -1 \\ 1
	\end{array}
	\right)\\
\text{Implicit form: } &\{ (x,y,z) | -3x -y + z = -2 \}\\
\text{Explicit form: } &\{ (-2 +s-t, s, t | s,t \in \mathbb{R} \}
\end{align*}

\begin{problem}{5.c}
\end{problem}
\begin{align*}
\vec u &= \left( \begin{array}{c}
	1 \\ -2 \\ 1
	\end{array}
	\right)\\
\text{Implicit form: } &\{ (x,y,z) | x = \frac{y - 1}{-2} = z + 1 \}\\
\text{Explicit form: } &\{ (t, -2t + 1, t - 1 | t \in \mathbb{R} \}
\end{align*}

\end{document}