\documentclass[12pt]{article}
\usepackage[margin=1in]{geometry} 
\usepackage{mathtools,amsmath,amsthm,amssymb,amsfonts}

\newcommand*\diff{\mathop{}\!\mathrm{d}}
\newcommand*\Diff[1]{\mathop{}\!\mathrm{d^#1}} 
\newcommand{\N}{\mathbb{N}}
\newcommand{\Z}{\mathbb{Z}}

\newenvironment{problem}[2][Problem]{\begin{trivlist}
\item[\hskip \labelsep{\bfseries #1}\hskip \labelsep{\bfseries #2.}]}{\end{trivlist}}

\begin{document}

\title{MA1104 Multivariable Calculus Assignment 4}
\author{Lim Wen Bin \\
	A0140764H\\
	T01}
\maketitle

\subsubsection*{Problem 1}
\begin{gather*}
	0 \le \phi \le \cos^{-1} (2/4) = \pi/3 \\
	z = \rho\cos\phi \\
	z \ge \rho\Rightarrow 2 \le \rho\cos\phi \\
	2/\cos\phi \le \rho\\
	\begin{align*}
		\iiint_E z(x^2+y^2+z^2)^{-3/2} dV 
			&= \int_0^{2\pi} \int_0^{\pi/3} \int_{2/\cos\phi}^{4} 
				\rho\cos\phi (\rho^2)^{-3/2} \cdot \rho^2 \sin\phi
			\diff\rho \diff\phi \diff\theta &\\
		&= \int_0^{2\pi} \diff\theta 
			\int_0^{\pi/3} \int_{2/\cos\phi}^{4} 
				\cos\phi \sin\phi
			\diff\rho \diff\phi \\
		&= 2\pi
			\int_0^{\pi/3}
				\Bigl[ \rho \cos\phi \sin\phi \Bigl]_{2/\cos\phi}^{4}  
			\diff\phi \\
		&= 2\pi \int_0^{\pi/3}
				2 \sin2\phi - 2 \sin\phi
			\diff\phi \\
		&= 2\pi \Bigl[ -\cos2\phi + 2\cos\phi \Bigl]_0^{\pi/3} \\
		&= 2\pi \Bigl[ 0.5 + 1 + 1 - 2\Bigl]\\
		&= \pi
	\end{align*}
\end{gather*}
\filbreak

\subsubsection*{Problem 2}
\begin{gather*}
	\intertext{Using polar coordinates,}
	\pi/6 \le \theta \le 5\pi/6 \\
	\intertext{For the circle $x^2 + (y-1)^2 = 1$,}
	(r\cos\theta)^2 + (r\sin\theta - 1)^2 = 1 \\
	(r\cos\theta)^2 + (r\sin\theta)^2 -2r\sin\theta + 1 = 1 \\
	r^2 -2r\sin\theta = 0 \\
	r(r -2\sin\theta) = 0 \\
	1 \le r \le 2\sin\theta \\
	\begin{align*}
		\iint_D x \diff A &= \int_{\pi/6}^{5\pi/6} \int_1^{2\sin\theta} 
			r\cos\theta \cdot r
		\diff r \diff \theta &\\
		&= \int_{\pi/6}^{5\pi/6}
			\Bigl[ \frac{1}{3} r^3 \cos\theta \Bigl]_1^{2\sin\theta} 
		\diff \theta \\
		&= \frac{1}{3} \int_{\pi/6}^{5\pi/6}
			 8 \sin^3\theta \cos\theta - \cos\theta
		\diff \theta \\
		&= \frac{1}{3} \Bigl[
			 2 \sin^4\theta - \sin\theta
		\Bigl]_{\pi/6}^{5\pi/6} \diff \theta \\
		&= \frac{1}{3} \Bigl[
			 \frac{1}{8} - \frac{1}{2} - \left(\frac{1}{8} - \frac{1}{2}\right)
		\Bigl] \\
		&= 0
	\end{align*}
\end{gather*}
\filbreak

\subsubsection*{Problem 3}
\begin{gather*}
	\intertext{Suppose the given integral is obtained after a transformation $T$ from the 
		$uv$ plane to the $xy$ plane.}
	\text{$u = \frac{y}{\sqrt{x}}$ and $v = x^2 + y^2$,} \\
	\begin{align*}
		\left| \frac{\partial (u,v)}{\partial (x,y)} \right| &= 
			\left| 
				\frac{\partial u}{\partial x} \frac{\partial v}{\partial y}
				- \frac{\partial u}{\partial y} \frac{\partial v}{\partial x}
			\right| &\\
		&= \left| -\frac{y}{2x^{3/2}}(2y) - \frac{1}{\sqrt{x}}(2x) \right| \\
		&= \left| -\frac{y^2}{x^{3/2}} - 2\sqrt{x} \right| \\
		&= \left| \frac{y^2}{x^{3/2}} + 2\sqrt{x} \right| \\
		&= \left| x^{-3/2} (y^2+ 2x^2) \right| \\
		\left| \frac{\partial (x,y)}{\partial (u,v)} \right| &= 
			\left| \frac{\partial (u,v)}{\partial (x,y)} \right|^{-1} \\
		\iint_D \frac{2x^2 + y^2}{xy} \diff A &= 
			\iint_D x^{-3/2}(2x^2 + y^2)\frac{\sqrt{x}}{y} \diff A \\
		&= \int_1^4 \int_1^2 u^{-1} \diff u \diff v \\
		&= \int_1^4 \diff v \Bigl[ \ln u \Bigl]_1^2 \\
		&= 3 \ln 2
	\end{align*}
\end{gather*}
\filbreak

\end{document}
