\documentclass[12pt]{article}
\usepackage[margin=1in]{geometry} 
\usepackage{mathtools,amsmath,amsthm,amssymb,amsfonts}

\newcommand*\diff{\mathop{}\!\mathrm{d}}
\newcommand*\Diff[1]{\mathop{}\!\mathrm{d^#1}} 
\newcommand{\N}{\mathbb{N}}
\newcommand{\Z}{\mathbb{Z}}
 
\newenvironment{problem}[2][Problem]{\begin{trivlist}
\item[\hskip \labelsep {\bfseries #1}\hskip \labelsep {\bfseries #2.}]}{\end{trivlist}}
 
\begin{document}

\title{MA1104 Multivariable Calculus Tutorial 2}
\author{Lim Wen Bin \\
A0140764H\\
T01}
\maketitle

\begin{problem}{1}
\end{problem}
\begin{align*}
\intertext{Let $n$ be the normal to the plane $3x + 2y -z = 6$.}
n &= \left( \begin{array}{c}
	3\\
	2\\
	-1\\
\end{array} \right) \\
L : X
&=
\left( \begin{array}{c}
	2\\
	3\\
	4\\
\end{array} \right)
+ s
\left( \begin{array}{c}
	3\\
	2\\
	-1\\
\end{array} \right)
, 
s \in \mathbb{R}
\end{align*}
\filbreak

\begin{problem}{2.a}
\end{problem}
\begin{align*}
L_1 : X &= 
\left( \begin{array}{c}
	2\\
	3\\
	4\\
\end{array} \right)
+ t
\left( \begin{array}{c}
	4\\
	0\\
	-1\\
\end{array} \right)
, 
t \in \mathbb{R} \\
L_2 : Y &= 
\left( \begin{array}{c}
	2\\
	3\\
	1\\
\end{array} \right)
+ s
\left( \begin{array}{c}
	2\\
	2\\
	1\\
\end{array} \right)
, 
s \in \mathbb{R} \\
\intertext{If $L_1$ and $L_2$ intersect,}
4t - 2s &= 0 \\
2s &= 0 \\
-t - s &= 0\\
\intertext{Solving for $s$ and $t$,}
t &= 0 \\
s &= 0 \\
\intertext{$L_1$ and $L_2$ intersect when $s=0$ and $t=0$.}
\end{align*}
\filbreak

\begin{problem}{2.b}
\end{problem}
\begin{align*}
L_1 : X &= 
\left( \begin{array}{c}
	1\\
	-2\\
	-1\\
\end{array} \right)
+ t
\left( \begin{array}{c}
	-3\\
	2\\
	4\\
\end{array} \right)
, 
t \in \mathbb{R} \\
L_2 : Y &= 
\left( \begin{array}{c}
	-2\\
	4\\
	3\\
\end{array} \right)
+ s
\left( \begin{array}{c}
	2\\
	4\\
	1\\
\end{array} \right)
, 
s \in \mathbb{R} \\
\intertext{If $L_1$ and $L_2$ intersect,}
-3t - 2s &= -3 \\
2t - 4s &= 6 \\
4t - s &= 4\\
\intertext{Solving for $s$ and $t$,}
t + (2/3)s &= 1 \\
s &= 0\\
0 &= 4 \\
\intertext{There is no solution and $L_1$ and $L_2$ do not intersect.}
\end{align*}
\filbreak

\begin{problem}{3}
\end{problem}
\begin{align*}
A &= (2, 2, 1)  \\
B &= (-1, 1, -1)  \\
\vec{AB} &= (-1, 1, -1) - (2, 2, 1)  \\
&= (-3, -1, -2)  \\
\intertext{Let $n$ be the normal to the required plane, $L$.}
n &= \left| \begin{array}{ccc}
	i & j & k\\
	-3 & -1 & -2\\
	2 & -3 & 1\\
\end{array} \right| \\
&= (-7, -1, 11)  \\
L : 
-7x -y +11z &= (-7, -1, 11) \cdot (-1, 1, -1)  \\
&= -5
\end{align*}
\filbreak

\begin{problem}{4}
\end{problem}
\begin{align*}
\intertext{Point $A (1, 0, 0)$ is on the plane $P$ with normal $n=(1,1,1)$.} 
\vec{QA} &= (1,0,0) - (2,1,2) \\
&= (-1,-1,-2)
\intertext{Let the point on the plane closest to $Q$ be $X$.} 
\vec{QX} &= \text{proj}_{n} \vec{QA} \\
&= \frac{-4}{3} (1,1,1) \\
X &= \frac{-4}{3} (1,1,1) + (2,1,2) \\
&= (2/3, -1/3, 2/3)\\
\end{align*}
\filbreak

\begin{problem}{5}
\end{problem}
\begin{gather*}
2x -3y +4z = 3, x +4y -2z = 7\\
2x = 3 +3y -4z , x = 7 -4y +2z \\
3 +3y -4z = 14 -8y +4z \\
11y = 11 + 8z \\
y = 1 + (8/11)z \\
x = 8 + (30/11)z \\
\therefore 
y = 1 + (8/11)s, x = 8 + (30/11)s, z = s, \forall s \in \mathhb{R} \\
\end{gather*}
\filbreak

\begin{problem}{6}
\end{problem}
\begin{align*}
\intertext{Let $L$ be the intersection of the planes.}
L : X &= a_L + s d_L , s \in \mathbb{R} \\
d_L &= (2,-3,1) \times (1,2,-3) \\
&= (7,7,7) \\
\intertext{To find $a_L$, suppose $z=0$,}
-3y + z &= 3 \\
2y + -3z &= 5 \\
\intertext{Solving for $y$ and $z$,}
y &= -2 \\
z &= -3 \\
L: X &= (0,-2,-3) + s(1,1,1)
\intertext{Let $n$ be the normal of the required plane, $P$.}
n &= (1,1,1) \times (3,2,-4) \\
&= (-6,7,-1) \\
P : -6x +7y -z &= (-6,7,-1) \cdot (0,-2,-3) \\
&= -11 \\ 
\end{align*}
\filbreak

\begin{problem}{7}
\end{problem}
\begin{align*}
\intertext{Point $A (1,1,0)$ lies on the plane.}
B &= (1,-2,4) \\
\vec{AB} &= (1,-2,4) - (1,1,0) \\
&= (0,-3,4) \\
\text{Distance} &= \frac{(0,-3,4) \cdot (3,2,6)}{7} \\
&= \frac{18}{7}
\end{align*}
\filbreak

\begin{problem}{8}
\end{problem}
\begin{align*}
2x -3y +z = 4 &\Rightarrow 4x -6y +2z = 8 \\
\text{Distance between planes} &= \frac{8-3}{2\sqrt{14}} \\
&= \frac{5}{2\sqrt{14}} \\
\end{align*}
\filbreak

\begin{problem}{9}
\end{problem}
\begin{proof}
\begin{align*}
\intertext{Let $A_P$ denote the area of the face opposite $P$.}
v_1 &= \lambda ((\vec{PQ} - \vec{PS}) \times (\vec{PR} - \vec{PS})) 
, \lambda \in \mathbb{R} \\
A_P &= \frac{1}{2} \lVert (\vec{PQ} - \vec{PS}) \times (\vec{PR} - \vec{PS}) \rVert \\
&= \lVert v_1 \rVert \\
\therefore v_1 &= \frac{1}{2} ((\vec{PQ} - \vec{PS}) \times (\vec{PR} - \vec{PS})) \\
\shortintertext{Similiarly,}
v_2 &= \frac{1}{2} (\vec{PS} \times \vec{PR}) \\
v_3 &= \frac{1}{2} (\vec{PQ} \times \vec{PS}) \\
v_4 &= \frac{1}{2} (\vec{PR} \times \vec{PQ}) \\
\shortintertext{Then,}
2\sum_{i=1}^{4} v_i &= 
((\vec{PQ} - \vec{PS}) \times (\vec{PR} - \vec{PS})) \\
&\phantom{=}+ (\vec{PS} \times \vec{PR}) 
+ (\vec{PQ} \times \vec{PS})
+ (\vec{PR} \times \vec{PQ}) \\
&= 
\vec{PQ} \times \vec{PR} - \vec{PQ} \times \vec{PS} - \vec{PS} \times \vec{PR} + 0 \\
&\phantom{=}+ (\vec{PS} \times \vec{PR}) 
+ (\vec{PQ} \times \vec{PS})
+ (\vec{PR} \times \vec{PQ}) \\
&= 
- \vec{PR} \times \vec{PQ} - \vec{PQ} \times \vec{PS} - \vec{PS} \times \vec{PR} + 0 \\
&\phantom{=}+ (\vec{PS} \times \vec{PR}) 
+ (\vec{PQ} \times \vec{PS})
+ (\vec{PR} \times \vec{PQ}) \\
&= 0
\end{align*}
\end{proof}
\filbreak

\end{document}
