\documentclass[12pt]{article}
\usepackage[margin=1in]{geometry} 
\usepackage{mathtools,amsmath,amsthm,amssymb,amsfonts}

\newcommand*\diff{\mathop{}\!\mathrm{d}}
\newcommand*\Diff[1]{\mathop{}\!\mathrm{d^#1}} 
\newcommand{\N}{\mathbb{N}}
\newcommand{\Z}{\mathbb{Z}}
 
\newenvironment{problem}[2][Problem]{\begin{trivlist}
\item[\hskip \labelsep {\bfseries #1}\hskip \labelsep {\bfseries #2.}]}{\end{trivlist}}
 
\begin{document}

\title{MA1102R Tutorial 11}
\author{Lim Wen Bin \\
A0140764H\\
T03}
\maketitle

\begin{problem}{1.b}
\end{problem}
\begin{align*}
\sqrt{x} \frac{dy}{dx} &= e^{y+\sqrt{x}}, \quad x, y > 0\\
y+\sqrt{x} &= \frac{1}{2}\ln x + \ln \frac{dy}{dx}\\
\ln \frac{dy}{dx}  &= y + \sqrt{x} - \frac{1}{2}\ln x\\
\frac{dy}{dx}  &= e^{\sqrt{x} - \frac{1}{2}\ln x } \cdot e^y\\
&= \frac{e^{- \sqrt{x}}}{\sqrt{x}} \cdot e^y\\
\int e^{-y} \diff y &= \int \frac{e^{- \sqrt{x}}}{\sqrt{x}} \diff x\\
&= -2\int -\frac{e^{- \sqrt{x}}}{2\sqrt{x}} \diff x\\
&= -2 e^{-\sqrt{x}}
\end{align*}
\filbreak

\begin{problem}{1.e}
\end{problem}
\begin{align*}
(t-1)^3\frac{ds}{dt} + 4(t-1)^2s &= t + 1, \quad t>1\\
\frac{ds}{dt} + \frac{4}{t-1}s &= \frac{t + 1}{(t-1)^3}\\
\intertext{Let $p(t) = \frac{4}{t-1}$, $q(t) = \frac{t+1}{(t-1)^3}$.}
\frac{ds}{dt} + p(t)s &= q(t)\\
\int \frac{4}{t-1} \diff t &= 4\ln(t-1) + C\\
P(t) &= 4\ln (t-1)\\
e^{P(t)}\frac{ds}{dt} + e^{P(t)}p(t)s &= e^{P(t)}q(t)\\
\frac{d}{dt}(e^{P(t)}s) &= e^{P(t)}q(t)\\
e^{P(x)}s &= \int e^{P(t)}q(t) \diff t\\
s &= \frac{1}{e^{P(t)}} \int e^{P(t)}q(t) \diff x\\
&= \frac{1}{(t-1)^4} \int \frac{(t+1)(t-1)^4}{(t-1)^3} \diff t\\
&= \frac{1}{(t-1)^4} \int (t+1)(t-1)\diff t\\
&= \frac{1}{(t-1)^4} (\frac{t^3}{3} - t + C)\\
\end{align*}
\filbreak

\begin{problem}{2.b}
\end{problem}
\begin{align*}
x\frac{dy}{dx} &= y + x^2\sin x, \quad x>0\\
\frac{dy}{dx} - \frac{1}{x}\cdot y &= x\sin x\\
\int -\frac{1}{x} &= -\ln x + C\\
\intertext{Let integrating factor $v(x) = e^(-\ln x) =x^{-1}$,}
y &= x \int \frac{x\sin x}{x} \diff x\\
&= x \int \sin x \diff x\\
&= x (-\cos x + C)\\
y(\pi) &= 0\\
\pi (-\cos \pi + C) &= 0\\
C &= \cos \pi\\
&= -1\\
y &= x (-\cos x - 1)\\
\end{align*}
\filbreak

\begin{problem}{3}
\end{problem}
\begin{align*}
\frac{dy}{dx} &= 4x^3y\\
\int \frac{1}{y} \diff y &= \int 4x^3\diff x\\
\ln y &= x^4 + C_1\\
y &= C_2 e^{x^4}\\
\intertext{When $x = 0$, $ y = 7$.}
7 &= C_2 e^0\\
C_2 &= 7\\
\text{$\therefore$ equation of curve}:y &= 7e^{x^4}
\end{align*}
\filbreak

\begin{problem}{5}
\end{problem}
\begin{align*}
\frac{dL}{dx} &= -kL\\
\int \frac{1}{L} \diff L &= \int -k \diff x\\
\ln L &= -kx + C_1\\
L &= C_2e^{-kx}\\
L(0) &= C_2e^0\\
&= C_2 \\
L(18) &= \frac{C_2}{2}\\
e^{-18k} &= \frac{1}{2}\\
\intertext{When intensity is one-tenth,}
(e^{-18k})^{\log_2 10} &= \left( \frac{1}{2} \right)^{\log_2 10}\\
x &= 18 \log_2 10\\ 
&= 59.79\\
&\approx 59.8
\end{align*}
\filbreak

\begin{problem}{7}
\end{problem}
\begin{align*}
\intertext{By Newton's Law of Cooling,}
\frac{dT}{dt} &= -r(T-T_S)\\
\int \frac{1}{T-T_S} \diff T &= \int -r \diff t\\
T - T_s &= Ce^{-rt}\\
46 - T_s &= C\\
39 - T_s &= Ce^{-10r}\\
39 - T_s &= (46 - T_s)e^{-10r}\\
\frac{39 - T_s}{46 - T_s} &= e^{-10r}\\
\frac{33 - T_s}{46 - T_s} &= e^{-20r}\\
\left(\frac{39 - T_s}{46 - T_s}\right)^2  &= \frac{33 - T_s}{46 - T_s}\\
(39 - T_s)^2 &= (33 - T_s)(46 - T_s)\\
(39 - T_s)^2 - (33 - T_s)(46 - T_s) &= 0
\intertext{Let $u = 39 - T_S$,}
u^2 - (u-6)(u+7) &= 0\\
-7u+6u+42 &= 0\\
u &= 42\\
39 - T_S &= 42\\
T_S &= 42 - 39\\
&= -3
\end{align*}
\filbreak

\end{document}