\documentclass[12pt]{article}
\usepackage[margin=1in]{geometry} 
\usepackage{amsmath,amsthm,amssymb,amsfonts}
 
\newcommand{\N}{\mathbb{N}}
\newcommand{\Z}{\mathbb{Z}}
 
\newenvironment{problem}[2][Problem]{\begin{trivlist}
\item[\hskip \labelsep {\bfseries #1}\hskip \labelsep {\bfseries #2.}]}{\end{trivlist}}
 
\begin{document}

\title{MA1102R Calculus Tutorial 7}
\author{Lim Wen Bin}
\maketitle
 
\begin{problem}{1.a}
\end{problem}
\begin{align*}
\lim_{x \to -3}\frac{t^3 -4t + 15}{t^2 -t - \sin(t)}
&= \lim_{x \to -3}\frac{3t^2 -4}{2t -1 - \cos(t)} \\
&= \frac{23}{-7 - \cos(-3)}
\end{align*}

\begin{problem}{1.b}
\end{problem}
\begin{align*}
\lim_{x \to 0} \frac{8x^2}{\cos(x) - 1} &=
\lim_{x \to 0} \frac{16x}{-\sin(x)} \\
&= \lim_{x \to 0} \frac{16}{-\cos(x)} \\
&= -16
\end{align*}

\begin{problem}{1.f}
\end{problem}
\begin{align*}
\lim_{x \to 1} \frac{\sqrt{3-x} - \sqrt{1+x}}{x^2 + x - 2}
&= \lim_{x \to 1} \frac{-(3-x)^{-1/2} - (1+x)^{-1/2}}{2x + 1}\\
&= \frac{-(2)^{-1/2} - (2)^{-1/2}}{3} \\
&= -\frac{\sqrt{2}}{3}
\end{align*}

\begin{problem}{1.g}
\end{problem}
\begin{align*}
\lim_{x \to a} \frac{x^m - a^m}{x^n - a^n} &=
\lim_{x \to a} \frac{mx^{m-1}}{nx^{n-1}} \\
&= \frac{m}{n}a^{m-n-2}\\
\end{align*}

\begin{problem}{2}
\end{problem}
\begin{align*}
\int_{0}^{a} x^3 dx &= \lim_{n \to \infty} \sum_{i=1}^{n} (\frac{i}{n})^3 \cdot \frac{a}{n} \\
&= \lim_{n \to \infty} \frac{a}{n^4} \sum_{i=1}^{n} i^3 \\
&= \lim_{n \to \infty}((\frac{n(n+1)}{2}) ^2 \cdot \frac{a}{n^4})\\
&= \frac{a}{4} \lim_{n \to \infty} \frac{n^4 + 2n^3 + n^2}{n^4}\\
&= \frac{a}{4}
\end{align*}

\begin{problem}{4.a}
\end{problem}
\begin{align*}
\intertext{Let $u = x^2$,}
\frac{dy}{dy} &= \frac{d}{dx} \int_{0}^{u} \cos(t^{1/3})dt \\
&= \frac{du}{dx} \cdot \frac{d}{du} \int_{0}^{u} \cos(t^{1/3})dt\\
&= 2x (\cos(x^{2/3}))
\end{align*}

\begin{problem}{4.b}
\end{problem}
\begin{align*}
\intertext{Let $u = x^{1/2}$,}
\frac{dy}{dy} &= \frac{d}{dx} \int_{\pi}^{x^{1/2}} \sin(t)dt \\
&= \frac{du}{dx} \cdot \frac{d}{du} \int_{\pi}^{x^{1/2}} \sin(t)dt\\
&= \frac{1}{2x^{1/2}} \sin(x^{1/2})
\end{align*}

\begin{problem}{5}
\end{problem}
\begin{align*}
F`(x) &=\frac{d}{dx}(\int_{g(x)}^{a} f(t)dt + \int_{a}^{h(x)} f(t)dt) \\
&= \frac{d}{dx}( \int_{a}^{h(x)} f(t)dt -\int_{a}^{g(x)} f(t)dt ) \\
&= h`(x) \cdot f(h(x)) - g`(x) \cdot f(g(x))\\
F``(x) &= h``(x)f(h(x)) + (h`(x))^2f(h(x)) - g``(x)f(g(x)) - (g`(x))^2f(g(x))
% \intertext{Let $g(x) = u, h(x) = v$,}
% F`(x) &=\frac{d}{dx} \int_{g(x)}^{h(x)} f(t)dt \\
% &= g`(x) \cdot \frac{d}{du} \int_{u}^{h(x)} f(t)dt \\
% &= g`(x) \cdot \frac{dv}{du} \cdot \frac{d}{dv} \int_{u}^{v} f(t)dt \\
% &= g`(x) \cdot \frac{h`(x)}{g`(x)} \cdot \frac{d}{dv} \int_{u}^{v} f(t)dt \\
% &= h`(x) f(v) dt \\
% &= h`(x) f(h(x)) dt
\end{align*}

\begin{problem}{6}
\end{problem}
\begin{align*}
F`(x) &= \frac{d}{dx} \int_{a}^{x} f(t)dt + \frac{d}{dx} \int_{a}^{x} tf(t)dt \\ 
&= \int_{a}^{x} f(t)dt + xf(x) - xf(x) \\
&= \int_{a}^{x} f(t)dt\\
F``(x) &= f(x)
\end{align*}

\end{document}