\documentclass[12pt]{article}
\usepackage[margin=1in]{geometry} 
\usepackage{amsmath,amsthm,amssymb,amsfonts}
 
\newcommand*\diff{\mathop{}\!\mathrm{d}}
\newcommand*\Diff[1]{\mathop{}\!\mathrm{d^#1}}
\newcommand{\N}{\mathbb{N}}
\newcommand{\Z}{\mathbb{Z}}
 
\newenvironment{problem}[2][Problem]{\begin{trivlist}
\item[\hskip \labelsep {\bfseries #1}\hskip \labelsep {\bfseries #2.}]}{\end{trivlist}}
 
\begin{document}

\title{MA1102R Calculus Tutorial 8}
\author{Lim Wen Bin}
\maketitle
 
\begin{problem}{1.c}
\end{problem}
\begin{align*}
\int \cos\theta (\tan\theta + \sec\theta) \diff \theta &= \int \sin\theta + \sec^2\theta \diff \theta\\
&= -\sin\theta + \tan\theta + C
\end{align*}

\begin{problem}{1.f}
\end{problem}
\begin{align*}
\int \csc x \diff x &= \int \frac{\csc x (-\cot x - \csc x)}{-\cot x - \csc x}\\
&= -\int \frac{-\csc^2 x - \csc\cot x}{\cot x + \csc x}\\
&= -\ln |\cot x + \csc x| + C
\end{align*}

\begin{problem}{1.g}
\end{problem}
\begin{align*}
&\int \sqrt{1+\sin^2 (x-1)} \sin(x-1) \cos(x-1) \diff x\\
&= \frac{2}{6} \int \frac{3}{2} \sqrt{1+\sin^2 (x-1)} \cdot 2\sin(x-1) \cos(x-1) \diff x\\
&= \frac{1}{3} (1+ \sin^2 (x-1))^{3/2} + C
\end{align*}

\begin{problem}{2.c}
\end{problem}
\begin{align*}
\intertext{Sub $u = 1 + \frac{1}{t}$, $\frac{du}{dt} = -t^{-2}$,}
\int_{-1}^{-1/2} t^{-2} \sin^2 (1 + \frac{1}{t}) \diff t &= -\int_{0}^{-1} \frac{t^{-2}}{t^{-2}} \sin^2 u \diff u\\
&= -\frac{1}{2} \int_{0}^{-1} 1 - \cos 2u \diff u\\
&= \frac{1}{4} \sin 2u - \frac{1}{2} u \biggl|_{0}^{-1}\\
&= \frac{1}{4} \sin (-2) + \frac{1}{2}\\
\end{align*}

\begin{problem}{2.d}
\end{problem}
\begin{align*}
\int_{2}^{4} \frac{dx}{x(\ln x)^2} &= -\int_{2}^{4} -\frac{dx}{x(\ln x)^2}\\
&= -\frac{1}{\ln x} \biggl|_{2}^{4}\\
&= -\frac{1}{\ln 4} + \frac{1}{\ln 2}\\
&= -\frac{1}{2\ln 2} + \frac{1}{\ln 2}\\
&= \frac{1}{2\ln 2}\\
\end{align*}

\begin{problem}{3.b}
\end{problem}
\begin{align*}
\intertext{$y$ is discontinuous at $x = {-2, 2}$. To find area between graph and $x$-axis for $x \in (-2,2)$, find:}
|\int_{-2}^{0} y \diff x| + \int_{0}^{2} y \diff x &= \frac{1}{3} \biggl[|-(4-x^2)^{3/2}|\biggl|_{-2}^{0} -(4-x^2)^{3/2} \biggl|_{0}^{2}\biggl]\\
&= \frac{1}{3} \biggl[|-(4)^{3/2}| +(4)^{3/2}\biggl]\\
&= \frac{16}{3} 
\end{align*}

\begin{problem}{4.b}
\end{problem}
\begin{align*}
\intertext{Sub. $u = \tan ^{-1} x$, $\frac{du}{dx} = \frac{1}{1 + x^2}$,}
\int_{0}^{\infty} \frac{16\tan^{-1}x}{1+x^2} \diff x &= \int_{0}^{\pi /2} 16u \diff u\\
&= \lim_{t \to \pi/2} \int_{0}^{t} 16u \diff u\\
&= \lim_{t \to \pi/2} 8u^2 \biggl|_{0}^{t} \\
&= \lim_{t \to \pi/2} 8t^2 \biggl|_{0}^{t} \\
&= 2\pi^2
\end{align*}

\begin{problem}{4.c}
\end{problem}
\begin{align*}
\int_{0}^{a} \frac{1}{x^{1/5}} \diff x &= \frac{5}{4x^{4/5}} \biggl|_{0}^{a} \\
&= \frac{5}{4a^{4/5}} 
\end{align*}

\begin{problem}{5.i}
\end{problem}
\begin{proof}
\begin{align*}
\intertext{Let $u = \pi - v$, $\frac{du}{dv} = -1$,}
\int_{0}^{\pi} vf(\sin v) \diff v &= -\int_{\pi}^{0} (\pi - u) f(\sin (\pi - u)) \diff u\\
&= \int_{0}^{\pi} (\pi - u) f(\sin (\pi - u)) \diff u\\
&= \pi \int_{0}^{\pi} f(\sin (\pi - u)) \diff u - \int_{0}^{\pi} u f(\sin (\pi - u)) \diff u\\
&= \pi \int_{0}^{\pi} f(\sin (\pi - u)) \diff u - \int_{0}^{\pi} u f(\sin (\pi - u)) \diff u\\
\intertext{Changing variables to $x$,}
2\int_{0}^{\pi} x f(\sin (\pi - x)) \diff x &= \pi \int_{0}^{\pi} f(\sin (\pi - x)) \diff x\\  
\int_{0}^{\pi} x f(\sin (\pi - x)) \diff x &= \frac{\pi}{2} \int_{0}^{\pi} f(\sin (\pi - x)) \diff x\\  
\end{align*}
\end{proof}

\begin{problem}{5.ii}
\end{problem}
\begin{align*}
\int_{0}^{\pi} \frac{x\sin x}{1 + \cos^2x} \diff x &= \int_{0}^{\pi} \frac{x\sin x}{2 - \sin^2x} \diff x \\
&= \frac{\pi}{2} \int_{0}^{\pi} \frac{\sin x}{2 - \sin^2x} \diff x\\
&= \frac{\pi}{2} \int_{0}^{\pi} \frac{\sin x}{1 + \cos^2x} \diff x\\
&= -\frac{\pi}{2} \int_{1}^{-1} \frac{1}{1 + u^2} \diff u \qquad \text{(Sub. $u = \cos x$, $\frac{du}{dx} = -\sin x$)}\\
&= -\frac{\pi}{2} \tan^{-1}u \biggl|_{1}^{-1} \\
&= -\frac{\pi}{2} [\tan^{-1} (-1) - \tan^{-1} 1]\\
&= \frac{\pi}{2} \cdot \frac{\pi}{2}\\
&= \frac{\pi^2}{4}
\end{align*}

\begin{problem}{6.b}
\end{problem}
\begin{align*}
f'(x) &= \frac{d}{dx} \sqrt{x^3 + x^2 + x + 1} \\
&= \frac{3x^2 + 2x + 1}{2\sqrt{x^3 + x^2 + x + 1}} \\
(f^{-1})'(x) &= \frac{2\sqrt{x^3 + x^2 + x + 1}}{3x^2 + 2x + 1} \\
(f^{-1})'(2) &= \frac{2\sqrt{2^3 + 2^2 + 2 + 1}}{3(2)^2 + 2(2) + 1} \\
(f^{-1})'(2) &= \frac{2\sqrt{8 + 4 + 2 + 1}}{17} \\
(f^{-1})'(2) &= \frac{2\sqrt{15}}{17} \\
\end{align*}

\begin{problem}{7.b}
\end{problem}
\begin{align*}
y &= \frac{x\sin x}{\sqrt{\sec x}}\\
\ln |y| &= \ln |x| + \ln|\sin x| - \frac{1}{2} \ln|{\sec x}|\\
\frac{1}{y} \frac{dy}{dx} &= \frac{1}{x} + \frac{\cos x}{\sin x} - \frac{\sec x \tan x}{2\sec x}\\
&= \frac{1}{x} + \cot x - \frac{1}{2}\tan x\\
\frac{dy}{dx} &= (\frac{1}{x} + \cot x - \frac{1}{2}\tan x)\frac{x\sin x}{\sqrt{\sec x}}
\end{align*}

\end{document}