\documentclass[12pt]{article}
\usepackage[margin=1in]{geometry} 
\usepackage{mathtools,amsmath,amsthm,amssymb,amsfonts}

\newcommand*\diff{\mathop{}\!\mathrm{d}}
\newcommand*\Diff[1]{\mathop{}\!\mathrm{d^#1}} 
\newcommand{\N}{\mathbb{N}}
\newcommand{\Z}{\mathbb{Z}}
 
\newenvironment{problem}[2][Problem]{\begin{trivlist}
\item[\hskip \labelsep {\bfseries #1}\hskip \labelsep {\bfseries #2.}]}{\end{trivlist}}
 
\begin{document}

\title{MA1102R Homework Assignment 3}
\author{Lim Wen Bin \\
A0140764H\\
T03}
\maketitle

\begin{problem}{1}
\end{problem}
\begin{align*}
\lim_{x \to 0} \left( \frac{\cos x}{\cos 2x} \right)^{1/x^2} &=
\lim_{x \to 0}
\text{exp}\left(\frac{\ln \cos x - \ln \cos 2x}{x^2}\right) 
\\
&=
\text{exp}\left(
\lim_{x \to 0}
\frac{\ln \cos x - \ln \cos 2x}{x^2}
\right) 
\\
&=
\text{exp}\left(
\lim_{x \to 0}
\frac{-\tan x + 2\tan 2x}{2x}
\right)
\\
&=
\text{exp}\left(
\lim_{x \to 0}
\frac{-\sec^2 x + 4\sec^2 2x}{2}
\right) 
\\
&=
\text{exp}\left(
\frac{3}{2}
\right) \\
&= e^{\frac{3}{2}}
\end{align*}
\filbreak

\begin{problem}{1.b}
\end{problem}
\begin{align*}
\lim_{x \to 0} \left( \frac{1+x2^x}{1+x3^x} \right)^{1/x^2} &=
\lim_{x \to 0}
\text{exp}\left(\frac{\ln(1+x2^x)-\ln(1+x3^x)}{x^2}\right) 
\\
&=
\text{exp}\left(
\lim_{x \to 0}
\frac{\ln(1+x2^x)-\ln(1+x3^x)}
{x^2}
\right)
\\
&=
\text{exp}\left[
\lim_{x \to 0}
\frac{1}{2x} 
\left(
\frac{2^x+x2^x\ln2}{1+x2^x} - \frac{3^x+x3^x\ln3}{1+x3^x}
\right)
\right] 
\\
&=
\text{exp}\biggl[
\lim_{x \to 0}
\frac{1}{2} 
\biggl(
\frac{2^x\ln2 + 2^x\ln2 + x2^x\ln2\ln2 - 2^x-x2^x\ln2} {(1+x2^x)^2} \\
&\phantom{=}- 
\frac{3^x\ln3 + 3^x\ln3 + x3^x\ln3\ln3 - 3^x-x3^x\ln3} {(1+x3^x)^2} 
\biggl)
\biggl] 
\\
&=
\text{exp}\biggl[
\lim_{x \to 0}
\frac{1}{2} 
\biggl(
\frac{2^x(\ln2 + \ln2 + x\ln2\ln2 - 1 -x\ln2)} {(1+x2^x)^2} \\
&\phantom{=}- 
\frac{3^x(\ln3 + \ln3 + x\ln3\ln3 - 1 -x\ln3)} {(1+x2^x)^2} 
\biggl)
\biggl] 
\\
&=
\text{exp}[
\frac{1}{2}(
(2\ln2 - 1)
- 
(2\ln3 - 1)
)]
\\
&=
\text{exp}(
\ln\frac{2}{3}
)\\
&= \frac{2}{3}
\end{align*}
\filbreak

\begin{problem}{2.a}
\end{problem}
\begin{align*}
\intertext{Let $u = x^{1/4}$, $\frac{du}{dx} = \frac{1}{4}x^{-3/4} = \frac{1}{4}u^{-3}$,}
\int e^{\sqrt[4]{x}} \diff x &= \int 4 u^3 e^u \diff u\\
&= 4 u^3 e^u - 12\int u^2 e^u \diff u + C_1\\
&= 4 u^3 e^u - 12 u^2 e^u + 24\int u e^u \diff u + C_2\\
&= 4 u^3 e^u - 12 u^2 e^u + 24u e^u - 24\int e^u \diff u + C_3\\
&= 4 u^3 e^u - 12 u^2 e^u + 24u e^u - 24e^u + C_4\\
&= 4 x^{3/4} e^{x^{1/4}} - 12 u^2 e^{x^{1/4}} + 24u e^{x^{1/4}} - 24e^{x^{1/4}}  + C_4\\
\end{align*}
\filbreak

\begin{problem}{2.b}
\end{problem}
\begin{align*}
\intertext{Let $x = 2\sec u$, $u \in [0,\frac{\pi}{2}] \cup [\pi, \frac{3\pi}{2})$, $\frac{dx}{du} = 2\sec u\tan u$, $u = \sec^{-1}\left(\frac{x}{2}\right)$,}
\int
	\frac{
		1
	}
	{
		x^3 \sqrt{x^2-4}
	}
\diff x
&=
\int
	\frac{
		2\sec u\tan u
	}
	{
		8\sec^3 u \sqrt{4\sec^2 u - 4}
	}
\diff u\\
&=
\int
	\frac{
		\sec u\tan u
	}
	{
		8\sec^3 u \tan u
	}
\diff u\\
&=
\frac{1}{8}
\int
	\cos^2 u
\diff u\\
&=
\frac{1}{8}
\int
	\frac{
		\cos 2u + 1
	}
	{
		2
	}
\diff u\\
&=
\frac{1}{16} 
\left(
\frac{\sin 2u}{2} + u
\right)
\\
&=
\frac{1}{16} 
\left(
\sin u \cos u + u
\right)
\\
&=
\frac{1}{16} 
\left(
\frac{2\sqrt{x^2-4}}{x^2} + \sec^{-1}\left(\frac{x}{2}\right)
\right)
\\
\end{align*}
\filbreak

\begin{problem}{2.c}
\end{problem}
\begin{align*}
\int 
	\frac{
		3
	}
	{
		x^3 - 1
	}
\diff x
&=
\int 
	\frac{
		3
	}
	{
		(x-1) (x^2+x+1)
	}
\diff x
\\
&=
\int 
	\frac{
		1
	}
	{
		x-1
	}
	-
	\frac{
		x+2
	}
	{
		x^2+x+1
	}
\diff x
\\
&=
\int 
	\frac{
		1
	}
	{
		x-1
	}
\diff x
-
\frac{1}{2}\int 
	\frac{
		2x+1
	}
	{
		x^2+x+1
	}
	+
	\frac{
		3
	}
	{
		(x+\frac{1}{2})^2 + \frac{3}{4}
	}
\diff x
\\
&=
\int 
	\frac{
		1
	}
	{
		x-1
	}
\diff x
-
\frac{1}{2}\int 
	\frac{
		2x+1
	}
	{
		x^2+x+1
	}
-
2\int 
	\frac{
		1
	}
	{
		\frac{4}{3} (x+\frac{1}{2})^2 + 1
	}
\diff x
\\
&=
\ln|x-1|
-
\frac{1}{2}\ln |x^2+x+1|
-
2 
\frac{\sqrt{3}}{2}
\tan^{-1} \left(
	\frac{2}{\sqrt{3}} (x+\frac{1}{2})
\right)
+ C
\\
&=
\ln|x-1|
-
\frac{1}{2}\ln |x^2+x+1|
-
\sqrt{3}
\tan^{-1} \left(
	\frac{2}{\sqrt{3}} (x+\frac{1}{2})
\right)
+ C
\end{align*}
\filbreak

\begin{problem}{3.i}
\end{problem}
\begin{proof}
\begin{align*}
\intertext{For $n \ge 1$,}
A_n 
&= 
\int_{0}^{\pi/2} 
	x^n \cos x
\diff x
\\
&=
\left[
	x^n \sin x
\right]_{0}^{\pi/2}
-
\int_{0}^{\pi/2} 
	n x^{n-1} \sin x
\diff x
\\
&=
\left(\frac{\pi}{2}\right)^n \sin \left(\frac{\pi}{2}\right)
- 0 -
n\int_{0}^{\pi/2} 
	x^{n-1} \sin x
\diff x
\\
&=
\left(\frac{\pi}{2}\right)^n 
- 
n B_{n-1}
\\
B_n 
&= 
\int_{0}^{\pi/2} 
	x^n \sin x
\diff x
\\
&=
\left[
	x^n \cos x
\right]_{0}^{\pi/2}
-
\int_{0}^{\pi/2} 
	n x^{n-1} \sin x
\diff x
\\
&=
0 - 0 -
n\int_{0}^{\pi/2} 
	x^{n-1} \sin x
\diff x
\\
&=
n A_{n-1}
\\
\end{align*}
\end{proof}
\filbreak

\begin{problem}{3.ii}
\end{problem}
\begin{align*}
A_0 &= \int_{0}^{\pi/2} \cos x \diff x\\
&= \left[\sin x\right]_{0}^{\pi/2}\\
&= 1\\
B_0 &= \int_{0}^{\pi/2} \sin x \diff x\\
&= \left[-\cos x\right]_{0}^{\pi/2}\\
&= 1\\
A_3 
&= 
\left(\frac{\pi}{2}\right)^3 
- 3B_{2}
\\
&= 
\left(\frac{\pi}{2}\right)^3 
- 3(2)A_{1}
\\
&= 
\left(\frac{\pi}{2}\right)^3 
- 3(2) \left[
	\left(\frac{\pi}{2}\right)
	- B_0
\right]
\\
&= 
\left(\frac{\pi}{2}\right)^3 
- 3(2) \left[
	\left(\frac{\pi}{2}\right)
	- 1
\right]
\\
&=
\frac{\pi^3}{8}
- 3 \pi
+ 6
\\
B_3 
&= 
3A_{2}
\\
&= 
3\left[
	\left(\frac{\pi}{2}\right)^2 
	- 2B_{1}
\right]
\\
&= 
3\left[
	\left(\frac{\pi}{2}\right)^2 
	- 2A_{0}
\right]
\\
&= 
3\left[
	\left(\frac{\pi}{2}\right)^2 
	- 2
\right]
\\
&=
3\left(\frac{\pi}{2}\right)^2 
- 6
\\
\end{align*}
\filbreak

\begin{problem}{4.a}
\end{problem}
\begin{align*}
\intertext{Washer method:}
\text{when } x &= 0,\\
y &= 0\\
\text{Volume} 
&= 
\int_{0}^{4} 
	\pi
	(\sqrt{x})^2
\diff x
\\
&= 
\int_{0}^{4} 
	\pi x
\diff x
\\
&= 
\left[
	\frac{
		\pi x^2
	}
	{
		2	
	}
\right]_{0}^{4}
\\
&= 
\frac{
	16\pi 
}
{
	2	
}
\\
&= 
8\pi 
\intertext{Cylindrical shell method:}
y &= \sqrt{x}\\
x &= y^2\\
\text{when } x &= 4,\\
y &= 2\\
\text{Volume} 
&= 
4(2)^2\pi
-
\int_{0}^{2} 
	2\pi
	y
	(y^2)
\diff y
\\
&= 
16\pi
-
\left[
	\frac{2\pi y^4}
	{4}
\right]_{0}^{2} 
\\
&= 
16\pi
-
\frac{2(16)\pi}
{4}
\\
&= 
16\pi
-
8\pi
\\
&=
8\pi
\end{align*} \filbreak

\begin{problem}{4.b}
\end{problem}
\begin{align*}
\intertext{Washer method:}
\text{Volume} 
&= 
2(4)^2\pi
-
\int_{0}^{2} 
	\pi
	(y^2)^2
\diff y
\\
&= 
32\pi
-
\left[
	\frac{
		\pi y^5
	}
	{5}
\right]_{0}^{2} 
\\
&= 
32\pi
-
\frac{
	32 \pi
}
{
	5	
}
\\
&=
\frac{
	128 \pi
}
{
	5	
}
\intertext{Cylindrical shell method:}
\text{Volume} 
&= 
\int_{0}^{4} 
	2\pi x \sqrt{x}
\diff x
\\
&= 
\left[
	\frac{4\pi y^{5/2}}
	{5}
\right]{0}^{4} 
\\
&= 
\frac{4\pi y^{5/2}}
{5}
\\
&= 
\frac{
	128 \pi
}
{
	5	
}
\end{align*}
\filbreak

\begin{problem}{4.c}
\end{problem}
\begin{align*}
\intertext{Washer method:}
\text{Volume} 
&= 
4 (3)^2 \pi 
-
\int_{0}^{4} 
	\pi
	(3 - \sqrt{x})^2
\diff x
\\
&= 
36\pi
-
\int_{0}^{4} 
	(9 - 6\sqrt{x} + x)
	\pi
\diff x
\\
&= 
36\pi
-
\left[
	(9x - 4x^{3/2} + \frac{x^2}{2})
	\pi
\right]_{0}^{4} 
\\
&= 
36\pi
-
12\pi
\\
&=
24 \pi 
\intertext{Cylindrical shell method:}
y &= 3 - \sqrt{x}\\
x &= (3 - y)^2\\
\text{Volume} 
&= 
4 (3)^2 \pi 
-
4 (1)^2\pi 
-
\int_{1}^{3} 
	2\pi y (3-y)^2
\diff y
\\
&= 
36 \pi 
-
4 \pi 
-
2\pi
\int_{1}^{3} 
	 9y - 6y^2 + y^3
\diff y
\\
&= 
32 \pi 
-
2\pi
\left[
	 \frac{9y^2}{2} - 2y^3 + \frac{y^4}{4}
\right]_{1}^{3} 
\\
&= 
32 \pi 
-
2(4)\pi
\\
&= 
24 \pi 
\end{align*}
\filbreak

\begin{problem}{4.d}
\end{problem}
\begin{align*}
\intertext{Washer method:}
\text{Volume} 
&= 
\int_{0}^{2} 
	\pi
	(y^2 - 5)^2
\diff y
-
2 (1)^2 \pi 
\\
&= 
\pi
\int_{0}^{2} 
	y^4 - 10y^2 + 25
\diff y
-
2 \pi 
\\
&= 
\pi
\left[
	\frac{y^5}{5} - \frac{10y^3}{3} + 25y
\right]_{0}^{2} 
-
2 \pi 
\\
&=
\pi
\left[
	\frac{2^5}{5} - \frac{10(2)^3}{3} + 25(2)
\right]
-
2 \pi 
\\
&= 
\frac{446\pi}{15}
-
2\pi
\\
&=
\frac{416\pi}{15} 
\intertext{Cylindrical shell method:}
\text{Volume} 
&= 
\int_{1}^{5} 
	2\pi x \sqrt{5 - x}
\diff x
\\
&= 
-2\pi 
\int_{4}^{0}
	(5 - u) \sqrt{u}
\diff u \quad (\text{sub. $u=5-x$, $\frac{du}{dx}=-1$})
\\
&= 
-2\pi 
\int_{4}^{0}
	5\sqrt{u} - u^{3/2} 
\diff u
\\
&= 
-2\pi 
\left[
	\frac{10u^{3/2}}{3} - \frac{2u^{5/2}}{5} 
\right]_{4}^{0} 
\\
&= 
2\pi 
\left[
	\frac{10(4)^{3/2}}{3} - \frac{2(4)^{5/2}}{5} 
\right]\\
&=
\frac{2(208)\pi}{15}\\
&=
\frac{416\pi}{15}
\end{align*}
\filbreak

\begin{problem}{5.a}
\end{problem}
\begin{align*}
\text{$(a, b)$ is a point on the graph} &\Rightarrow \text{$(a, -b)$ is a point on the graph}\\
&\Rightarrow \text{$(-a, b)$ is a point on the graph}\\
\intertext{$\therefore$ The graph is symmetric about the $x$-axis and $y$-axis.}
x = 0 &\Rightarrow y = 1\\
y = 0 &\Rightarrow x = 1\\
\intertext{In the first quadrant,}
y &= (1 - x^{2/3})^{3/2}\\
\frac{dy}{dx}
&=
-\frac{3}{2} \left(\frac{2}{3}\right) x^{-1/3}
(1 - x^{2/3})^{1/2}
\\
&=
-(x^{-2/3}(1 - x^{2/3}))^{1/2}
\\
&=
-(x^{-2/3} - 1)^{1/2}
\\
\text{Length of curve} 
&=
4 \int_{0}^{1}
	\sqrt{
		1 + (x^{-2/3} - 1)
	}
\diff x
\\
&=
4 \int_{0}^{1}
	x^{-1/3}
\diff x
\\
&=
4 \left[
	\frac{3x^{2/3}}{2}
\right]_{0}^{1}
\\
&=
4 \left(
	\frac{3(1)^{2/3}}{2}
\right)
\\
&= 6 
\end{align*}
\filbreak

\begin{problem}{5.b}
\end{problem}
\begin{align*}
\frac{dx}{dy}
&=
\frac{1}{2} \sqrt{y^2-1}
+
\frac{y^2}
{2\sqrt{y^2-1}}
-
\frac{
	1 + y(y^2-1)^{-1/2}
}
{
	2(y+(y^2-1)^{1/2})
}
\\
&=
\frac{1}{2} \sqrt{y^2-1}
+
\frac{y^2}
{2\sqrt{y^2-1}}
-
\frac{
	1
}
{
	2(y^2-1)^{1/2}
}
\\
&=
\frac{
	y^2 - 1 + y^2 - 1
}
{
	2(y^2-1)^{1/2}
}
\\
&=
\frac{
	2(y^2 - 1)
}
{
	2(y^2-1)^{1/2}
}
\\
&=
\frac{
	(y^2 - 1)
}
{
	(y^2-1)^{1/2}
}
\\
&=
(y^2-1)^{1/2}
\\
\text{Length of curve}
&=
\int_{1}^{2}
	\sqrt{1 + y^2 - 1}
\diff y
\\
&=
\int_{1}^{2}
	y
\diff y
\\
&=
\left[
	\frac{y^2}{2}
\right]_{1}^{2}
\\
&=
\frac{2^2}{2}
-
\frac{1^2}{2}
\\
&=
\frac{3}{2}
\end{align*}
\filbreak

\begin{problem}{6.a}
\end{problem}
\begin{align*}
\frac{dy}{dx} 
&=
\frac{1}{2}(y^{-1/2} - y^{1/2})\\
&=
\frac{1 - y}{2y^{1/2}}\\
\text{Area of surface} 
&=
\int_{1}^{3} 
	2\pi 
	(y^{1/2}-\frac{1}{3}y^{3/2})
	\sqrt{
		1 + \frac{(1 - y)^2}{4y}
	}
\diff y
\\
&=
2\pi 
\int_{1}^{3} 
	(y^{1/2}-\frac{1}{3}y^{3/2})
	\sqrt{
		\frac{4y + (1 - y)^2}{4y}
	}
\diff y
\\
&=
2\pi 
\int_{1}^{3} 
	(y^{1/2}-\frac{1}{3}y^{3/2})
	\sqrt{
		\frac{(1 + y)^2}{4y}
	}
\diff y
\\
&=
2\pi 
\int_{1}^{3} 
	(y^{1/2}-\frac{1}{3}y^{3/2})
	\frac{1 + y}{2y^{1/2}}
\diff y
\\
&=
\pi 
\int_{1}^{3} 
	(1-\frac{1}{3}y)
	(1 + y)
\diff y
\\
&=
\pi 
\int_{1}^{3} 
	1-\frac{1}{3}y + y - \frac{1}{3}y^2
\diff y
\\
&=
\pi 
\int_{1}^{3} 
	1 + \frac{2}{3}y - \frac{1}{3}y^2
\diff y
\\
&=
\pi 
\left[
	y + \frac{1}{3}y^2 - \frac{1}{9}y^3
\right]_{1}^{3} 
\\
&=
\pi 
\left[
	3 + \frac{9}{3} - \frac{27}{9}
	-1 - \frac{1}{3} + \frac{1}{9}
\right]
\\
&=
\frac{
	16\pi
}
{
	9
}
\end{align*}
\filbreak

\begin{problem}{6.b}
\end{problem}
\begin{align*}
\frac{x^2}{25}
+
\frac{y^2}{16}
&=
1
\intertext{In the first and second quadrant,}
\left(
	\frac{y}{4}
\right)^2
&=
	1 -
\left(
	\frac{x}{5}
\right)^2
\\
y &=
4\sqrt{
	1 -
	\left(
		\frac{x}{5}
	\right)^2
}
\\
\frac{dy}{dx} &=
-\frac{
	4x 
}
{
	5(5)\sqrt{
		1 -
		\left(
			\frac{x}{5}
		\right)^2
	}
}
\\
&=
-\frac{
	4x 
}
{
	5\sqrt{
		25 - x^2
	}
}
\\
& \int
	2 \pi
	\cdot
	4\sqrt{
		1 -
		\left(
			\frac{x}{5}
		\right)^2
	}
	\sqrt{
		1+
		\frac{
			16x^2 
		}
		{
			25(25 - x^2)
		}
	}
\diff x
\\
&=
8 \pi
\int
	\sqrt{
		1 -
		\left(
			\frac{x}{5}
		\right)^2
	}
	\sqrt{
		\frac{
			25(25 - x^2) +
			16x^2 
		}
		{
			25(25 - x^2)
		}
	}
\diff x
\\
&=
8 \pi
\int
	\sqrt{
		\frac{
			(1 - \frac{x^2}{25})
			(625 - 9x^2)
		}
		{
			25(25 - x^2)
		}
	}
\diff x
\\
&=
8 \pi
\int
	\sqrt{
		\frac{
			625 - 25x^2
			- 9x^2 + \frac{9x^4}{25}
		}
		{
			25(25 - x^2)
		}
	}
\diff x
\\
&=
8 \pi
\int
	\sqrt{
		\frac{
			15625 - 850x^2 + 9x^4
		}
		{
			625(25 - x^2)
		}
	}
\diff x
\\
&=
8 \pi
\int
	\sqrt{
		\frac{
			(25 - x^2)(625 - 9x^2)
		}
		{
			625(25 - x^2)
		}
	}
\diff x
\\
&=
8 \pi
\int
	\sqrt{
		1 - \frac{9x^2}{625}
	}
\diff x
\\
&=
8 \left(\frac{25}{3}\right) \pi
\int
	\cos u \cos u 
\diff u
\quad (\text{
	sub. $\sin u = \frac{3}{25}x$, 
	$\frac{dx}{du} = \frac{25}{3}\cos u$, 
	$u \in [-\frac{\pi}{2}, \frac{\pi}{2}]$
})
\\
&=
8 \left(\frac{25}{3}\right) \pi
\int
	\frac{1+\cos2u}{2}
\diff u
\\
&=
8 \left(\frac{25}{3}\right) \pi
\left(
	\frac{u}{2} + \frac{\sin2u}{4}
\right)
+ C
\\
&= 
8 \left(\frac{25}{3}\right) \pi
\left(
	\frac{1}{2}\sin^{-1} \left(\frac{3x}{25}\right) + \frac{3x}{50} \sqrt{1-\frac{9x^2}{625}}
\right)
+ C
\\
&= 
8 \left(\frac{25}{3}\right) \pi
\left(
	\frac{1}{2}\sin^{-1} \left(\frac{3x}{25}\right) + \frac{3x}{1250} \sqrt{625-9x^2}
\right)
+ C
\end{align*}
\begin{align*}
y = 0 &\Rightarrow x = \pm 5\\
\text{Area of surface} &= 
8 \left(\frac{25}{3}\right) \pi
\left[
	\frac{1}{2}\sin^{-1} \left(\frac{3x}{25}\right) + \frac{3x}{1250} \sqrt{625-9x^2}
\right]_{-5}^{5}
\\
&= 235.3 \\
&\approx 235 \text{ units}^2 \quad (\text{$3$ s.f.})
\end{align*}
\filbreak

\end{document}