\documentclass[12pt]{article}
\usepackage[margin=1in]{geometry} 
\usepackage{mathtools,amsmath,amsthm,amssymb,amsfonts}

\newcommand*\diff{\mathop{}\!\mathrm{d}}
\newcommand*\Diff[1]{\mathop{}\!\mathrm{d^#1}} 
\newcommand{\N}{\mathbb{N}}
\newcommand{\Z}{\mathbb{Z}}
 
\newenvironment{problem}[2][Problem]{\begin{trivlist}
\item[\hskip \labelsep {\bfseries #1}\hskip \labelsep {\bfseries #2.}]}{\end{trivlist}}
 
\begin{document}

\title{PC2134 Assignment 1}
\author{Lim Wen Bin \\
A0140764H\\
Group 1}
\maketitle

\begin{problem}{1}
\end{problem}
\begin{align*}
	x(t) = u_0t,&\quad y(t) = v_0t - \frac{1}{2}gt^2\\
	x'(t) = u_0,&\quad y'(t) = v_0 - gt\\
	\theta(t) &= \tan^{-1}\frac{y'(t)}{x'(t)}\\
	&= \tan^{-1}\frac{v_0 - gt}{u_0}\\
	\shortintertext{The speed of the projectile is given by}
	v(t) &= (u_0^2 + (v_0-gt)^2)^{1/2}\\
	\shortintertext{while the kinetic energy of the projectile is}
	K(t) &= \frac{1}{2}m[v(t)]^2\\
	&= \frac{1}{2}m(u_0^2 + (v_0-gt)^2).\\
	\shortintertext{Then,}
	K'(t) &= -gm(v_0-gt)\\
\end{align*}

\begin{problem}{2.a}
\end{problem}
\begin{proof}
\begin{align*}
	\shortintertext{Integrating by parts,}
	I_{2n+1} &= \int_0^\infty x^{2n} \cdot x e^{-x^2} dx\\
	&= \frac{1}{2} (2n) \int_0^\infty x^{2n-2} \cdot x e^{-x^2} dx 
		- \left[ \frac{1}{2} x^{2n}e^{-x^2} \right]_0^\infty\\
	&= n \int_0^\infty x^{2n-2} \cdot x e^{-x^2} dx \quad 
		\left(\because \lim_{a\to 0} \left[ \frac{1}{2} x^{2n}e^{-x^2} \right]_0^a =
		0\right)\\
\end{align*}
\filbreak
\begin{align*}
	\shortintertext{Continuing for a total of $n$ times,}
	I_{2n+1} &= n! \int_0^\infty x e^{-x^2} dx\\
	&= n! \left[ \frac{1}{2} e^{-x^2} \right]_0^\infty\\
	&= \lim_{a\to0} n! \left[ \frac{1}{2} e^{-x^2} \right]_0^a\\
	&= \frac{n!}{2}
\end{align*}
\end{proof}

\begin{problem}{2.b}
\end{problem}
\begin{proof}
\begin{align*}
	\shortintertext{Integrating by parts,}
	I_{2n} &= \int_0^\infty x^{2n-1} \cdot x e^{-x^2} dx\\
	&= \frac{1}{2} (2n-1) \int_0^\infty x^{2n-2} e^{-x^2} dx 
		- \left[ \frac{1}{2} x^{2n-2} e^{-x^2} \right]_0^\infty\\
	&= 2^{-1} (2n-1) \int_0^\infty x^{2n-2} e^{-x^2} dx \quad 
		\left(\because \lim_{a\to0} \left[ \frac{1}{2} x^{2n-1}e^{-x^2} \right]_0^a =
		0\right)\\
	&= 2^{-1} (2n-1) I_{2n-2}
	\shortintertext{Continuing for a total of $n$ times,}
	I_{2n} &= 2^{-n} (2n-1)(2n-3)\ldots(3)(1) I_0
\end{align*}
\end{proof}

\begin{problem}{3}
\end{problem}
\begin{align*}
	a(t) &= \begin{cases}
		\frac{2g}{1-0.1t} - g, &0\le t \le 5\\
		- g, &5 < t\\
	\end{cases}
	\shortintertext{For $0\le t \le 5$,}
	v(t) &= \int \frac{2g}{1-0.1t} - g\ dt\\
	&= -20g \ln(1-0.1t) - gt + C\\
	v(0) = 0 &\Rightarrow C = 0\\
	v(5) &= 86.945\\
	\shortintertext{For $5< t,}
	v(t) &= \int -g\ dt = -gt + C\\
	v(5) = 86.945 &= -9.81(5) + C \Rightarrow C = 135.99\\
	\therefore v(t) &= \begin{cases}
		-g(20 \ln(1-0.1t) + t), &0\le t \le 5\\
		- gt + 135.99, &5 < t\\
	\end{cases}
\end{align*}
At the maximum height $h_m$, $v=0$, $t = \frac{135.99}{9.81} = 13.862$.
\begin{align*}
	h_m &= \int_0^5 -g(20 \ln(1-0.1t) + t)\ dt 
		+ \int_5^{13.862} - gt + 135.99\ dt\\
	&= - 20g \left( \left[ t\ln(1-0.1t) \right]_0^5
			+ \int_0^5 \frac{t}{10(1-0.1t)}  dt \right) 
			- \left[\frac{gt^2}{2}\right]_0^5
			+ \left[ -\frac{gt^2}{2} + 135.99t \right]_5^{13.862}\\
	&= 679.98
			- 2g\int_0^5 \frac{t}{1-0.1t}\ dt 
			- 122.63 + 385.24 \\
	&= 942.59 - 20g\int_0^5 \frac{t}{10-t}\ dt  \\
	&= 942.59 - 20g\int_0^5 -1 + \frac{10}{10-t}\ dt  \\
	&= 942.59 - 20g\left[ -t - 10\ln(10-t) \right]_0^5 \\
	&= 942.59 - 378.95 \approx 564\ (3\text{ s.f.})\\
\end{align*}

\begin{problem}{4}
\end{problem}
\begin{align*}
	y'(x) &= -\frac{x}{\sqrt{1-x^2}}\\
	l &= \int_0^1 \sqrt{1+y'(x)^2}\ dx\\
	&= \int_0^1 \sqrt{1 + \frac{x^2}{1-x^2}}\ dx\\
	&= \int_0^1 \sqrt{\frac{1-x^2+x^2}{1-x^2}}\ dx\\
	&= \int_0^1 \frac{1}{\sqrt{1-x^2}}\ dx\\
	&= \left[ \sin^{-1}(x) \right]_0^1  \\
	&= \frac{\pi}{2}
	\shortintertext{The resulting shape is a hemisphere.}
	A &= \frac{1}{2} \cdot 4 \pi (1)^2 \\
	&= 2 \pi \\
	V &= \frac{4}{3(2)}  \pi (1)^3 \\
	&= \frac{2\pi}{3} \\
	S &= A + \pi (1)^2 \\
	&= 2 \pi + 1\\
\end{align*}

\begin{problem}{5}
\end{problem}
\begin{align*}
	\shortintertext{The period of a single oscillation of the ball with some
		initial velocity $u$ is given by}
	t &= \frac{2u}{g}.
	\shortintertext{After $n$ bounces, the energy of the ball is}
	E_n &= E_0 \gamma^n. \\
	\shortintertext{Equivalently, by the relation $E_k = \frac{1}{2}mv^2$,
		after $n$ bounces, the initial upward velocity of the ball is}
	v_n &= v_0 \gamma^{n/2}. \\
	\shortintertext{The period of the $n$th bounce, for $n\ge0$, is therefore}
	t_n &= \frac{2v_0\gamma^{n/2}}{g}. \\
	T_\infty &= \frac{2v_0}{g} \sum_{i=0}^\infty (\sqrt{\gamma})^n
	\shortintertext{For small $\gamma$,}
	T_\infty &= \frac{2v_0}{g(1-\sqrt{\gamma})}.
\end{align*}

\end{document}
