\documentclass[12pt]{article}
\usepackage[margin=1in]{geometry} 
\usepackage{mathtools,amsmath,amsthm,amssymb,amsfonts}

\newcommand*\diff{\mathop{}\!\mathrm{d}}
\newcommand*\Diff[1]{\mathop{}\!\mathrm{d^#1}} 
\newcommand{\N}{\mathbb{N}}
\newcommand{\Z}{\mathbb{Z}}
 
\newenvironment{problem}[2][Problem]{\begin{trivlist}
\item[\hskip \labelsep {\bfseries #1}\hskip \labelsep {\bfseries #2.}]}{\end{trivlist}}
 
\begin{document}

\title{PC2134 Assignment 10}
\author{Lim Wen Bin \\
A0140764H\\
Group 1}
\maketitle

\begin{problem}{1.a}
\end{problem}
\begin{align*}
	\mathcal{L} \{ \cosh(at) \cos(at) \}
	&= \mathcal{L} \left\{ 
		\frac{e^{at} + e^{-at}}{2}
		\cdot
		\frac{e^{iat} + e^{-iat}}{2}
	\right\} \\
	&= \frac{1}{4} \mathcal{L} \{ 
		e^{(1+i)at} + e^{(i-1)at}
		+ e^{(1-i)at} + e^{(-1-i)at}
	\} \\
	&= \frac{1}{4} \left[
		\frac{1}{s-(1+i)a}
		+ \frac{1}{s-(i-1)a}
		+ \frac{1}{s-(1-i)a}
		+ \frac{1}{s+(i+1)a}
	\right]
\end{align*}

\begin{problem}{1.b}
\end{problem}
\begin{align*}
	\mathcal{L} \{ \cosh(at) \cos(at) \}
	&= \mathcal{L} \left\{ 
		\frac{e^{at} - e^{-at}}{2}
		\cdot
		\frac{e^{iat} - e^{-iat}}{2}
	\right\} \\
	&= \frac{1}{4} \mathcal{L} \{ 
		e^{(1+i)at} - e^{(i-1)at}
		- e^{(1-i)at} + e^{(-1-i)at}
	\} \\
	&= \frac{1}{4} \left[
		\frac{1}{s-(1+i)a}
		- \frac{1}{s-(i-1)a}
		- \frac{1}{s-(1-i)a}
		+ \frac{1}{s+(i+1)a}
	\right]
\end{align*}

\begin{problem}{2.a}
\end{problem}
\begin{align*}
	\mathcal{L}^{-1} \left\{ \frac{k^2}{s(s^2+k^2)} \right\}
	&= k \mathcal{L}^{-1} \left\{ \frac{1}{s} \left( \frac{k^2}{s^2+k^2}
		\right) \right\} \\
	&= k \int_0^t \sin(ku) \diff u
\end{align*}
\filbreak

\begin{problem}{2.b}
\end{problem}
\begin{gather*}
	\frac{s}{(s^2+a^2)(s^2+b^2)} 
		=
		\frac{As + B}{s^2+a^2}
		+ \frac{Cs + D}{s^2+b^2}
	\\
	(As+B) (s^2+b^2) + (Cs+D) (s^2+a^2) = s \\
	Bb^2 + Da^2 = 0 \\
	\intertext{Set $B = D = 0$.}
	As^3 + Cs^3 = 0 \Rightarrow A = -C \\
	Ab^2 + Ca^2 = 1 \\
	A = \frac{1}{b^2-a^2},\ B = \frac{1}{a^2-b^2} \\
	\begin{aligned}
		\therefore \mathcal{L}^{-1} \left\{ \frac{s}{(s^2+a^2)(s^2+b^2)} \right\}
		&= \mathcal{L}^{-1} \left\{ 
			\frac{s}{(b^2-a^2)(s^2+a^2)} 
			+
			\frac{s}{(a^2-b^2)(s^2+b^2)} 
		\right\} \\
		&= 
			\frac{1}{b^2-a^2} 
			\mathcal{L}^{-1} \left\{ 
				\frac{s}{s^2+a^2} 
			\right\} 
			+
			\frac{1}{a^2-b^2} 
			\mathcal{L}^{-1} \left\{ 
				\frac{s}{s^2+b^2} 
			\right\} 
		\\
		&= 
			\frac{1}{b^2-a^2} 
			\cos(at)
			+
			\frac{1}{a^2-b^2} 
			\cos(bt)
	\end{aligned}
\end{gather*}

\begin{problem}{3.a}
\end{problem}
\begin{gather*}
	m \frac{\diff^2 x(t)}{\diff t^2} + b \frac{\diff x(t)}{\diff t} + kx(t) = 0 \\
	\intertext{Taking the Laplace transform,}
	m \mathcal{L} \left\{ \frac{\diff^2 x}{\diff t^2} \right\}
		+ b \mathcal{L} \left\{ \frac{\diff x}{\diff t} \right\}
		+ k\bar{x}(s) = 0 .
	\\
	m \left[ 
			s^2\bar{x}(s) - sx(t) - \frac{\diff x(t)}{\diff t} 
		\right]_{t=0}
		+ b \left[ 
			s\bar{x}(s) - sx(t)
		\right]_{t=0}
		+ k\bar{x}(s) = 0
	\\
	m s^2\bar{x}(s) - m v_0 
		+ b s\bar{x}(s)
		+ k\bar{x}(s) = 0
	\\
	\bar{x}(s) = \frac{m v_0}{
		ms^2 + bs + k
	}
	\intertext{Completing the square,}
	\bar{x}(s) = \frac{v_0}{
		\left( s + \frac{b}{2m} \right)^2
		+
		\left( \frac{k}{m} - \frac{b^2}{4m^2} \right)
	}.
	\intertext{(i) For the underdamped system, $\frac{k}{m} - \frac{b^2}{4m^2}
	> 0$.}
	\mathcal{L}^{-1} \{ \bar{x}(s) \} 
		= 
		v_0
		\text{exp} \left(
			-\frac{b}{2m} t
		\right)
		\left( 
			\frac{k}{m} - \frac{b^2}{4m^2}
		\right)^{-1/2}
		\sin \left(
			t\sqrt{\frac{k}{m} - \frac{b^2}{4m^2}}
		\right)
	\intertext{(iii) For the overdamped system, $\frac{k}{m} - \frac{b^2}{4m^2}
	< 0$.}
	\mathcal{L}^{-1} \{ \bar{x}(s) \} 
		= 
		v_0
		\text{exp} \left(
			-\frac{b}{2m} t
		\right)
		\left( 
			\frac{b^2}{4m^2} - \frac{k}{m} 
		\right)^{-1/2}
		\sinh \left(
			t\sqrt{\frac{b^2}{4m^2} - \frac{k}{m}}
		\right)
\end{gather*}
\filbreak
\begin{gather*}
	\intertext{(ii) For the critically damped system, $\frac{k}{m} - \frac{b^2}{4m^2}
	= 0$.}
	\mathcal{L}^{-1} \{ \bar{x}(s) \} 
		= 
		\text{exp} \left(
			-\frac{b}{2m} t
		\right)
		\frac{v_0t}{2}
\end{gather*}

\begin{problem}{3.b}
\end{problem}
\begin{gather*}
	m \frac{\diff^2 x(t)}{\diff t^2} + b \frac{\diff x(t)}{\diff t} + kx(t)
		+ k\bar{x}(s) = 0 \\
	\intertext{Taking the Laplace transform,}
	m s^2\bar{x}(s) - m v_0 
		+ b s\bar{x}(s)
		+ k\bar{x}(s) 
		=
		\frac{F_0 \omega}{s^2 + \omega^2}.
	\\
	\bar{x}(s) = \frac{m v_0}{
			ms^2 + bs + k
		}
		+
		\frac{F_0 \omega}{(s^2 + \omega^2)(ms^2 + bs + k)}
	\\
	\begin{aligned}
	g(t) &:= 
		\mathcal{L}^{-1} \left\{
			\frac{m v_0}{ ms^2 + bs + k }
		\right\}
	\\
	&= 
		v_0
		\text{exp} \left(
			-\frac{b}{2m} t
		\right)
		\left( 
			\frac{k}{m} - \frac{b^2}{4m^2}
		\right)^{-1/2}
		\sin \left(
			t\sqrt{\frac{k}{m} - \frac{b^2}{4m^2}}
		\right)
	\end{aligned}
	\\
	x(t) = 
		g(t)
		+
		\mathcal{L}^{-1} \left\{ 
			\frac{F_0 \omega}{(s^2 + \omega^2)(ms^2 + bs + k)}
		\right\}
	\\
	\intertext{By the Laplace convolution theorem,}
	\mathcal{L}^{-1} \left\{
			F_0
			\frac{\omega}{s^2 + \omega^2}
			\cdot
			\frac{1}{ms^2 + bs + k}
		\right\}
		= 
		\frac{F_0}{mv_0} \sin(\omega t) \ast g(t).
	\\
	\therefore x(t) = 
		g(t)
		+
		\frac{F_0}{mv_0} \sin(\omega t) \ast g(t)
	\\
\end{gather*}

\end{document}
