\documentclass[12pt]{article}
\usepackage[margin=1in]{geometry} 
\usepackage{mathtools,amsmath,amsthm,amssymb,amsfonts}
\usepackage{braket}

\newcommand*\diff{\mathop{}\!\mathrm{d}}
\newcommand*\Diff[1]{\mathop{}\!\mathrm{d^#1}} 
\newcommand{\N}{\mathbb{N}}
\newcommand{\Z}{\mathbb{Z}}
 
\newenvironment{problem}[2][Problem]{\begin{trivlist}
\item[\hskip \labelsep {\bfseries #1}\hskip \labelsep {\bfseries #2.}]}{\end{trivlist}}
 
\begin{document}

\title{PC2134 Assignment 11}
\author{Lim Wen Bin \\
A0140764H\\
Group 1}
\maketitle

\begin{problem}{1}
\end{problem}
\begin{gather*}
	\braket{1|1} = \int_0^\infty e^{-x} \diff x 
		= [ -e^{-x} ]_0^\infty = 1 
	\\
	\hat{\phi}_0 = 1 \qed \\
	\braket{x|\hat{\phi}_0} = \int_0^\infty xe^{-x} \diff x 
		= \int_0^\infty e^{-x} \diff x 
		= [ -e^{-x} ]_0^\infty = 1 
	\\
	\phi_1 = x - 1 \\
	\begin{aligned}
		\braket{\phi_1|\phi_1} &= \int_0^\infty (x-1)^2 e^{-x} \diff x \\
		&= \int_0^\infty (x^2 - 2x + 1) e^{-x} \diff x \\
		&= \int_0^\infty 2 x e^{-x} \diff x - 1 \\
		&= 2 - 1 = 1
	\end{aligned} \\
	\hat{\phi}_1 = x-1 \qed \\
	\braket{x^2|\hat{\phi}_0} = \int_0^\infty x^2 e^{-x} \diff x = 2 \\
	\braket{x^2|\hat{\phi}_1} = \int_0^\infty x^2 (x-1) e^{-x} \diff x 
		= 6 - 2  = 4 \\
	\phi_2 = x^2 - 4(x-1) - 2 = x^2 - 4x + 2 \\
	\begin{aligned}
		\braket{\phi_2|\phi_2} &= \int_0^\infty (x^2 - 4x + 2)^2 e^{-x} \diff x \\
		&= \int_0^\infty (x^4 - 8x^3 + 20x^2 - 16x + 4) e^{-x} \diff x \\
		&= 24 - 8(6) + 20(2) - 16 + 4 = 4 \\
	\end{aligned} \\
	\hat{\phi}_2 = \frac{1}{2}(x^2 - 4x + 2) \qed
\end{gather*}

\begin{problem}{2}
\end{problem}
For $w(x) = 1$,
\begin{gather*}
	\mathcal{L} = \frac{\diff}{\diff x^2} + \kappa \\
	\mathcal{L}\phi(x) = \lambda \phi(x) \\
	\frac{\diff^2 \phi}{\diff x^2} + \kappa \phi = \lambda \phi
		\Rightarrow \frac{\diff^2 \phi}{\diff x^2} + (\kappa - \lambda) \phi = 0 \\
	\phi(x) = c_1 \cos(x \sqrt{\kappa - \lambda}) 
		+ c_2 \sin(x \sqrt{\kappa - \lambda}) \\
	\phi(0) = 0 \Rightarrow c_1 = 0 \\
	\phi(\pi) = 0 \Rightarrow \sin(\pi \sqrt{\kappa - \lambda}) = 0 \\
	\lambda_n = \kappa - n^2,\quad n \in \mathbb{Z}^+ \cup \{0\} \\
	\phi_n(x) = c_2 \sin (nx) \\
	\braket{\phi_n|\phi_n} = \int_0^\pi \phi_n^* (x) \phi_n \diff x = c_2^2
		\frac{\pi}{2} \\
	\hat{\phi}_n (x) = \sqrt{\frac{2}{\pi}} \sin(nx) \\
	G(x, x') 
		= \sum_{n=0}^\infty 
			\frac{1}{\lambda_n} 
			\hat{\phi}_n^* (x') \hat{\phi}_n (x)
		= \frac{2}{\pi}
			\sum_{n=0}^\infty 
			\frac{\sin(nx') \sin(nx)}
			{\kappa - n^2} 
	\\
	\begin{aligned}
		y(x) &= \int_0^\pi G(x, x') f(x') \diff x' \\
		\frac{\pi}{2} y(x) &= \int_0^{\frac{\pi}{2}} 
				\sum_{n=0}^\infty 
				\frac{\sin(nx') \sin(nx)}
				{\kappa - n^2} 
				x'
			\diff x'
			+ \int_{\frac{\pi}{2}}^\pi 
				\sum_{n=0}^\infty 
				\frac{\sin(nx') \sin(nx)}
				{\kappa - n^2} 
				(\pi - x')
			\diff x'
		\\
		&= 
			\sum_{n=0}^\infty 
			\frac{\sin(nx)}
			{n(\kappa - n^2)} 
			\left\{
				\left[ - \cos(nx') x' \right]_0^{\frac{\pi}{2}}
				+
				\int_0^{\frac{\pi}{2}} 
					\cos(nx')
				\diff x'
			\right\}
			\\
			&\phantom{=}+
			\sum_{n=0}^\infty 
			\frac{\sin(nx)}
			{n(\kappa - n^2)} 
			\left\{
				\left[ - \cos(nx') (\pi - x') \right]_{\frac{\pi}{2}}^\pi
				+
				\int_{\frac{\pi}{2}}^\pi
					\cos(nx')
				\diff x'
			\right\}
		\\
		&= 
			\sum_{n=0}^\infty 
			\frac{\sin(nx)}
			{n(\kappa - n^2)} 
			\left[
				\left( \frac{\pi}{2} -1 \right)
				\cos \left( \frac{n\pi}{2} \right)
			\right]
		\\
		y(x) &= 
			\left( 1- \frac{2}{\pi} \right)
			\sum_{n=0}^\infty 
			\frac{\sin(nx)}
			{n(\kappa - n^2)} 
			\left[
				\cos \left( \frac{n\pi}{2} \right)
			\right]
		\\
		&= 
			\left( 1- \frac{2}{\pi} \right)
			\sum_{n=0}^\infty 
			\frac{\sin(2nx)}
			{2n(\kappa - 4n^2)} 
			(-1)^n
		\\
	\end{aligned}
	\\
\end{gather*}
\filbreak

\begin{problem}{3}
\end{problem}
The two dimension wave equation is given by
\begin{gather*}
	\frac{1}{v^2} \frac{\partial^2 \psi(x,y,t)}{\partial t^2}
		- \frac{\partial^2 \psi(x,y,t)}{\partial x^2}
		- \frac{\partial^2 \psi(x,y,t)}{\partial y^2}
		= 0. \\
	\intertext{Substituting the seperable form, $\psi(x,y,t) = X(x)Y(y)T(t)$, into the
	equation,}
	\frac{1}{v^2} \frac{1}{T(t)} \frac{\diff^2 T(t)}{\diff t^2}
		- \frac{1}{X(x)} \frac{\diff^2 X(x)}{\diff x^2}
		- \frac{1}{Y(x)} \frac{\diff^2 Y(y)}{\diff y^2}
		= 0. \\
	\intertext{For constants $-u^2$, $-v^2$ and $-w^2 = -u^2 - v^2$,}
	\frac{1}{X(x)} \frac{\diff^2 X(x)}{\diff x^2} = -u^2,\
	\frac{1}{Y(x)} \frac{\diff^2 Y(y)}{\diff y^2} = -v^2,\
	\frac{1}{v^2} \frac{1}{T(t)} \frac{\diff^2 T(t)}{\diff t^2} = -w^2. \\
	X(x) = U_1 \cos (ux) + U_2 \sin(ux),\
	Y(x) = V_1 \cos (vy) + V_2 \sin(vy),\
	T(x) = W_1 \cos (wvt) + W_2 \sin(wvt) \\
	\intertext{The boundary conditions are given as follows}
	\begin{cases}
		BC1: & \psi(0,y,t) = 0, \\
		BC2: & \psi(a,y,t) = 0, \\
		BC3: & \psi(x,0,t) = 0, \\
		BC4: & \psi(x,b,t) = 0, \\
		BC5: & \psi(x,y,0) = 
			\sin\left( \frac{\pi x}{a} \right)
			\sin\left( \frac{\pi y}{b} \right). \\
	\end{cases} \\
	\intertext{For $m, n \in \mathbb{Z}^+$,}
	(BC1) \land (BC2) \Rightarrow A_1 = 0,\ u_n = \frac{n\pi}{a}, \\
	(BC3) \land (BC4) \Rightarrow B_1 = 0,\ v_n = \frac{m\pi}{b}. \\
	w_{n,m} = \sqrt{
		\left( \frac{n\pi x}{a} \right)^2
		+ \left( \frac{m\pi y}{b} \right)^2
	} \\
	\begin{aligned}
		\psi(x,y,t) &= 
			\sum_{n,m} \left( 
				U_{n,m} \sin \left( \frac{n\pi x}{a} \right)
			\right) 
			\left( 
				V_{n,m} \sin \left( \frac{m\pi y}{b} \right)
			\right) 
			\left( 
				W_{n,m} \cos (w_{n,m}vt) + W_{n,m}' \sin(w_{n,m}vt)
			\right) \\
		&= \sum_{n,m} 
			\sin \left( \frac{n\pi x}{a} \right)
			\sin \left( \frac{m\pi y}{b} \right)
			\left[ 
				S_{n,m} \cos (w_{n,m}vt) + T_{n,m} \sin(w_{n,m}vt)
			\right] \\
	\end{aligned}
	\\
	\intertext{For $i, j > 1$,}
	(BC5) \Rightarrow S_{1,1} = 1,\ S_{i,j} = 0. \\
	\therefore \psi(x,y,t) = 
			\sum_{n=1}^\infty \sum_{m=1}^\infty
			\sin \left( \frac{n\pi x}{a} \right)
			\sin \left( \frac{m\pi y}{b} \right)
			\left( 
				\delta_{n,1} \delta_{m,1} \cos (w_{n,m}vt) + T_{n,m} \sin(w_{n,m}vt)
			\right) \\
\end{gather*}

\end{document}
