\documentclass[12pt]{article}
\usepackage[margin=1in]{geometry} 
\usepackage{mathtools,amsmath,amsthm,amssymb,amsfonts}

\newcommand*\diff{\mathop{}\!\mathrm{d}}
\newcommand*\Diff[1]{\mathop{}\!\mathrm{d^#1}} 
\newcommand{\N}{\mathbb{N}}
\newcommand{\Z}{\mathbb{Z}}
 
\newenvironment{problem}[2][Problem]{\begin{trivlist}
\item[\hskip \labelsep {\bfseries #1}\hskip \labelsep {\bfseries #2.}]}{\end{trivlist}}
 
\begin{document}

\title{PC2134 Assignment 5}
\author{Lim Wen Bin \\
A0140764H\\
Group 1}
\maketitle

\begin{problem}{1}
\end{problem}
For the stone to be always moving away from the thrower, the projection of the
velocity vector onto the position vector has to be a non-negative multiple of
the position vector. Or equivalently,
\[\mathbf{r} \cdot \mathbf{\dot{r}} > 0. \]
\intertext{For a stone thrown at angle $\theta$ from the horizontal,}
\begin{gather*}
	\mathbf{\dot{r}} = \left(\begin{array}{c} 
			v\cos\theta \\
			v\sin\theta - at \\
		\end{array} \right), \\
	\mathbf{r} = \left(\begin{array}{c} 
			vt\cos\theta \\
			vt\sin\theta - \frac{at^2}{2} \\
		\end{array} \right). \\
	\begin{aligned}
		\mathbf{r} \cdot \mathbf{\dot{r}} &= vt\cos^2\theta + (v\sin\theta-at)
			\left(vt\sin\theta-\frac{at^2}{2}\right) \\
		&= v^2t\cos^2\theta + v^2t\sin^2\theta  - avt^2\sin\theta -
			\frac{1}{2}avt^2\sin\theta + \frac{1}{2}a^2t^3 \\
		&= t \left( v^2 - \frac{3}{2}avt\sin\theta + \frac{1}{2}a^2t^2 \right) \\ 
		&=  \frac{a^2t}{2} \left( \frac{2v^2}{a^2} - \frac{3v\sin\theta}{a}t +
			t^2 \right) \\ 
		&=  \frac{a^2t}{2} \left[ 
			\frac{2v^2}{a^2} - \left(\frac{3v\sin\theta}{2a}\right)^2 + \left(t
			- \frac{3v\sin\theta}{2a}\right)^2
			\right] \\ 
	\end{aligned}
	\\
	\Rightarrow \frac{2v^2}{a^2} - \left(\frac{3v\sin\theta}{2a}\right)^2 > 0 \\
	\frac{2v^2}{a^2} > \frac{9v^2\sin^2\theta}{4a^2} \\
	2 > \frac{9\sin^2\theta}{4} \\
\end{gather*}
\begin{gather*}
	\frac{8}{9} > \sin^2\theta \\
	\sin\theta < \frac{2^{3/2}}{3} \\
	\theta < \sin^{-1} \frac{2^{3/2}}{3} \\
\end{gather*}
\filbreak

\begin{problem}{2}
\end{problem}
\begin{gather*}
	\mathbf{r} = \left( \begin{array}{c}
			r\sin\theta\cos\phi \\
			r\sin\theta\sin\phi \\
			r\cos\theta \\
		\end{array} \right) \\
	\frac{\partial\mathbf{r}}{\partial r} = \left( \begin{array}{c}
			\sin\theta\cos\phi \\
			\sin\theta\sin\phi \\
			\cos\theta \\
		\end{array} \right),\ 
		\frac{\partial\mathbf{r}}{\partial \theta} = \left( \begin{array}{c}
			r\cos\theta\cos\phi \\
			r\cos\theta\sin\phi \\
			-r\sin\theta \\
		\end{array} \right),\ 
		\frac{\partial\mathbf{r}}{\partial \phi} = \left( \begin{array}{c}
			-r\sin\theta\sin\phi \\
			r\sin\theta\cos\phi \\
			0 \\
		\end{array} \right) \\
	\left| \frac{\partial\mathbf{r}}{\partial r} \right| = 1,\ 
		\left| \frac{\partial\mathbf{r}}{\partial \theta} \right| = r,\ 
		\left| \frac{\partial\mathbf{r}}{\partial \phi} \right| = r\sin\theta \\
	\hat{\mathbf{e}}_r = \left( \begin{array}{c}
			\sin\theta\cos\phi \\
			\sin\theta\sin\phi \\
		\cos\theta \\
		\end{array} \right),\ 
		\hat{\mathbf{e}}_\theta = \left( \begin{array}{c}
			\cos\theta\cos\phi \\
			\cos\theta\sin\phi \\
			-\sin\theta \\
		\end{array} \right),\ 
		\hat{\mathbf{e}}_\phi = \left( \begin{array}{c}
			-\sin\phi \\
			\cos\phi \\
			0 \\
		\end{array} \right) \\
	\mathbf{r} \cdot \hat{\mathbf{e}}_r = r\sin^2\theta\cos^2\phi +
		r\sin^2\theta\sin^2\phi + r\cos^2\theta = r\\
	\mathbf{r} \cdot \hat{\mathbf{e}}_\theta = r\sin\theta\cos\theta\cos^2\phi +
		r\sin\theta\cos\theta\sin^2\phi - r\sin\theta\cos\theta = 0\\
	\mathbf{r} \cdot \hat{\mathbf{e}}_\phi = -r\sin\theta\sin\phi\cos\phi +
		r\sin\theta\sin\phi\cos\phi = 0\\
	\intertext{Let $\beta$ represent the orthogonal spherical basis. Then,}
	\mathbf{r} = \left( \begin{array}{c}
			r \\
			0 \\
			0 \\
		\end{array} \right)_\beta. \\
	\dot{\mathbf{r}} = \left( \begin{array}{c}
			\dot{r}\sin\theta\cos\phi +
			r\dot{\theta}\cos\theta\cos\phi -
			r\dot{\phi}\sin\theta\sin\phi \\
			\dot{r}\sin\theta\sin\phi +
			r\dot{\theta}\cos\theta\sin\phi +
			r\dot{\phi}\sin\theta\cos\phi \\
			\dot{r}\cos\theta - r\dot{\theta}\sin\theta \\
		\end{array} \right) \\
	\begin{aligned}
		\dot{\mathbf{r}} \cdot \hat{\mathbf{e}}_r &= 
			\sin\theta\cos\phi (\dot{r}\sin\theta\cos\phi +
				r\dot{\theta}\cos\theta\cos\phi - r\dot{\phi}\sin\theta\sin\phi) \\
			&\phantom{=}+ \sin\theta\sin\phi (\dot{r}\sin\theta\sin\phi +
				r\dot{\theta}\cos\theta\sin\phi + r\dot{\phi}\sin\theta\cos\phi) \\
			&\phantom{=}+ \cos\theta (\dot{r}\cos\theta - r\dot{\theta}\sin\theta) \\
		&= \dot{r}\sin^2\theta + r\dot{\theta}\sin\theta\cos\theta
			+ \dot{r}\cos^2\theta - r\dot{\theta}\sin\theta\cos\theta \\
		&= \dot{r}
	\end{aligned}
\end{gather*}
\filbreak
\begin{gather*}
	\begin{aligned}
		\dot{\mathbf{r}} \cdot \hat{\mathbf{e}}_\theta &= 
			\cos\theta\cos\phi (\dot{r}\sin\theta\cos\phi +
				r\dot{\theta}\cos\theta\cos\phi - r\dot{\phi}\sin\theta\sin\phi) \\
			&\phantom{=}+ \cos\theta\sin\phi (\dot{r}\sin\theta\sin\phi +
				r\dot{\theta}\cos\theta\sin\phi + r\dot{\phi}\sin\theta\cos\phi) \\
			&\phantom{=}- \sin\theta (\dot{r}\cos\theta - r\dot{\theta}\sin\theta) \\
		&= \dot{r}\sin\theta\cos\theta + r\dot{\theta}\cos^2\theta
			- \dot{r}\sin\theta\cos\theta + r\dot{\theta}\sin^2\theta \\
		&= r\dot{\theta} \\
		\dot{\mathbf{r}} \cdot \hat{\mathbf{e}}_\phi &= 
			-\sin\phi (\dot{r}\sin\theta\cos\phi +
				r\dot{\theta}\cos\theta\cos\phi - r\dot{\phi}\sin\theta\sin\phi) \\
			&\phantom{=}+ \cos\phi (\dot{r}\sin\theta\sin\phi +
				r\dot{\theta}\cos\theta\sin\phi + r\dot{\phi}\sin\theta\cos\phi) \\
		&= r\dot{\phi}\sin\theta
	\end{aligned} \\
	\therefore \mathbf{v} = \dot{\mathbf{r}} = \left( \begin{array}{c}
			\dot{r} \\
			r\dot{\theta} \\
			r\dot{\phi}\sin\theta \\
		\end{array} \right)_\beta \\
	\begin{aligned}
		[\ddot{\mathbf{r}}]_1 &= 
			\ddot{r}\sin\theta\cos\phi + \dot{r}\dot{\theta}\cos\theta\cos\phi
				- \dot{r}\dot{\phi}\sin\theta\sin\phi \\
			&\phantom{=} + \dot{r}\dot{\theta}\cos\theta\cos\phi 
				+ r\ddot{\theta}\cos\theta\cos\phi - r\dot{\theta}^2\sin\theta\cos\phi 
				- r\dot{\theta}\dot{\phi}\cos\theta\sin\phi \\
			&\phantom{=}- \dot{r}\dot{\phi}\sin\theta\sin\phi
				- r\dot{\theta}\dot{\phi}\cos\theta\sin\phi 
				- r\ddot{\phi}\sin\theta\sin\phi - r\dot{\phi}^2\sin\theta\cos\phi \\
		&= \ddot{r}\sin\theta\cos\phi 
				+ r\ddot{\theta}\cos\theta\cos\phi - r\dot{\theta}^2\sin\theta\cos\phi 
				- r\ddot{\phi}\sin\theta\sin\phi - r\dot{\phi}^2\sin\theta\cos\phi  \\
			&\phantom{=} 
				+ 2\dot{r}\dot{\theta}\cos\theta\cos\phi
				- 2\dot{r}\dot{\phi}\sin\theta\sin\phi 
				- 2r\dot{\theta}\dot{\phi}\cos\theta\sin\phi \\
		[\ddot{\mathbf{r}}]_2 &= 
			\ddot{r}\sin\theta\sin\phi + \dot{r}\dot{\theta}\cos\theta\sin\phi
				+ \dot{r}\dot{\phi}\sin\theta\cos\phi \\
			&\phantom{=} + \dot{r}\dot{\theta}\cos\theta\sin\phi 
				+ r\ddot{\theta}\cos\theta\sin\phi - r\dot{\theta}^2\sin\theta\sin\phi 
				+ r\dot{\theta}\dot{\phi}\cos\theta\cos\phi \\
			&\phantom{=}+ \dot{r}\dot{\phi}\sin\theta\cos\phi
				+ r\dot{\theta}\dot{\phi}\cos\theta\cos\phi 
				+ r\ddot{\phi}\sin\theta\cos\phi - r\dot{\phi}^2\sin\theta\sin\phi \\
		&= \ddot{r}\sin\theta\sin\phi 
				+ r\ddot{\theta}\cos\theta\sin\phi - r\dot{\theta}^2\sin\theta\sin\phi 
				+ r\ddot{\phi}\sin\theta\cos\phi - r\dot{\phi}^2\sin\theta\sin\phi  \\
			&\phantom{=} 
				+ 2\dot{r}\dot{\theta}\cos\theta\sin\phi
				+ 2\dot{r}\dot{\phi}\sin\theta\cos\phi 
				+ 2r\dot{\theta}\dot{\phi}\cos\theta\cos\phi \\
		[\ddot{\mathbf{r}}]_3 &= 
			\ddot{r}\cos\theta - 2\dot{r}\dot{\theta}\sin\theta 
			- r\ddot{\theta}\sin\theta - r\dot{\theta}^2\cos\theta \\
		\ddot{\mathbf{r}} \cdot \hat{\mathbf{e}}_r &= 
				\ddot{r}\sin^2\theta
				+ r\ddot{\theta}\sin\theta\cos\theta - r\dot{\theta}^2\sin^2\theta
				- r\dot{\phi}^2\sin^2\theta + 2\dot{r}\dot{\theta}\sin\theta\cos\theta \\
			&\phantom{=} 
				+ \ddot{r}\cos^2\theta - 2\dot{r}\dot{\theta}\sin\theta\cos\theta 
				- r\ddot{\theta}\sin\theta\cos\theta - r\dot{\theta}^2\cos^2\theta \\
			&= \ddot{r} - r\dot{\theta}^2 - r\dot{\phi}^2\sin^2\theta \\
		\ddot{\mathbf{r}} \cdot \hat{\mathbf{e}}_\theta &= 
				\ddot{r}\sin\theta\cos\theta
				+ r\ddot{\theta}\cos^2\theta - r\dot{\theta}^2\sin\theta\cos\theta
				- r\dot{\phi}^2\sin\theta\cos\theta + 2\dot{r}\dot{\theta}\cos^2\theta \\
			&\phantom{=} 
				-\ddot{r}\sin\theta\cos\theta + 2\dot{r}\dot{\theta}\sin^2\theta 
				+ r\ddot{\theta}\sin^2\theta + r\dot{\theta}^2\sin\theta\cos\theta \\
			&= r\ddot{\theta} - r\dot{\phi}^2\sin\theta\cos\theta +
				2\dot{r}\dot{\theta} \\
		\ddot{\mathbf{r}} \cdot \hat{\mathbf{e}}_\phi &= 
			r\ddot{\phi}\sin\theta + 2\dot{r}\dot{\phi}\sin\theta
			+ 2r\dot{\theta}\dot{\phi}\cos\theta \\
	\end{aligned} \\
	\therefore \mathbf{a} = \ddot{\mathbf{r}} = \left( \begin{array}{c}
			\ddot{r} - r\dot{\theta}^2 - r\dot{\phi}^2\sin^2\theta \\
			r\ddot{\theta} - r\dot{\phi}^2\sin\theta\cos\theta +
				2\dot{r}\dot{\theta} \\
			r\ddot{\phi}\sin\theta + 2\dot{r}\dot{\phi}\sin\theta
			+ 2r\dot{\theta}\dot{\phi}\cos\theta \\
		\end{array} \right)_\beta \\
\end{gather*}

\begin{problem}{3.a}
\end{problem}
\begin{align*}
	r &= \sqrt{x^2 + y^2 + z^2} \\
	\nabla \left( \frac{1}{r} \right) &= \left( \begin{array}{c}
			- x/r^3 \\
			- y/r^3 \\
			- z/r^3 \\
		\end{array} \right)
\end{align*}

\begin{problem}{3.b}
\end{problem}
\begin{align*}
	\nabla \cdot \left( \frac{\hat{\mathbf{r}}}{r^2} \right) &= 
		\nabla \cdot \left( \frac{\mathbf{r}}{r^3} \right) \\
	&= ( x/r^3 )_x + ( y/r^3 )_y + ( z/r^3 )_z \\
	&= \frac{r^2 - 3x^2}{r^5} + \frac{r^2 - 3y^2}{r^5} + \frac{r^2 - 3z^2}{r^5} \\
	&= \frac{3r^2-3r^2}{r^5} \\
	&= 0
\end{align*}

\begin{problem}{3.c}
\end{problem}
\begin{align*}
	\nabla \times \left( \frac{\hat{\mathbf{r}}}{r^2} \right) &= 
		\nabla \times \left( \frac{\mathbf{r}}{r^3} \right) \\
	&= -\nabla \times \left( -\frac{\mathbf{r}}{r^3} \right) \\
	&= -\nabla \times \left[ \nabla \left( \frac{1}{r} \right) \right] \\
	&= \mathbf{0}
\end{align*}

\begin{problem}{3.d}
\end{problem}
\begin{align*}
	\nabla^2 \left( \frac{1}{r} \right) &= 
		\nabla \cdot \left[ \nabla \left( \frac{1}{r} \right) \right] \\
	&= \nabla \cdot \left( -\frac{\hat{\mathbf{r}}}{r^2} \right) \\
	&= -\nabla \cdot \left( \frac{\hat{\mathbf{r}}}{r^2} \right) \\
	&= 0
\end{align*}
\filbreak

\begin{problem}{4}
\end{problem}
\begin{proof}
\begin{gather*}
	\mathbf{B} = \nabla \times \mathbf{A} \\
	\shortintertext{Taking curl on both sides,}
	\nabla \times \mathbf{B} = \nabla \times (\nabla \times \mathbf{A}). \\
	\frac{1}{c^2} \frac{\partial \mathbf{E}}{\partial t} = \nabla (\nabla \cdot
		\mathbf{A}) - \nabla^2 \mathbf{A} \\
	\nabla^2 \mathbf{A} + \frac{1}{c^2} \frac{\partial \mathbf{E}}{\partial t}
		+ \nabla \left( \frac{1}{c^2} \frac{\partial \Phi}{\partial t} \right) = 0 \\
	\nabla^2 \mathbf{A} + \frac{1}{c^2} \left[ \frac{\partial}{\partial t} \left(
		- \nabla \Phi - \frac{\partial A}{\partial t} \right) + 
		\nabla \frac{\partial \Phi}{\partial t} \right] = 0 \\
	\nabla^2 \mathbf{A} + \frac{1}{c^2} \left[ -\nabla \frac{\partial
		\Phi}{\partial t} - \frac{\partial^2 A}{\partial t^2} 
		+ \nabla \frac{\partial \Phi}{\partial t} \right] = 0 \\
	\nabla^2 \mathbf{A} - \frac{1}{c^2} \frac{\partial^2 A}{\partial t^2} = 0 \\
	\shortintertext{Next, we have}
	\mathbf{E} = - \nabla \Phi - \frac{\partial \mathbf{A}}{\partial t}. \\
	\shortintertext{Taking divergence on both sides,}
	\nabla \cdot \mathbf{E} = - \nabla^2 \Phi - \nabla \cdot \frac{\partial
		\mathbf{A}}{\partial t}. \\
	\nabla^2 \Phi + \nabla \cdot \frac{\partial \mathbf{A}}{\partial t} = 0 \\
	\nabla^2 \Phi + \frac{\partial }{\partial t} (\nabla \cdot \mathbf{A}) = 0 \\
	\nabla^2 \Phi + \frac{\partial }{\partial t} \left(- \frac{1}{c^2}
		\frac{\partial \Phi}{\partial t} \right) = 0 \\
	\nabla^2 \Phi - \frac{1}{c^2} \frac{\partial^2 \Phi}{\partial t^2} = 0 \\
\end{gather*}
\end{proof}

\end{document}

