\documentclass[12pt]{article}
\usepackage[margin=1in]{geometry} 
\usepackage{mathtools,amsmath,amsthm,amssymb,amsfonts}

\newcommand*\diff{\mathop{}\!\mathrm{d}}
\newcommand*\Diff[1]{\mathop{}\!\mathrm{d^#1}} 
\newcommand{\N}{\mathbb{N}}
\newcommand{\Z}{\mathbb{Z}}
 
\newenvironment{problem}[2][Problem]{\begin{trivlist}
\item[\hskip \labelsep {\bfseries #1}\hskip \labelsep {\bfseries #2.}]}{\end{trivlist}}
 
\begin{document}

\title{PC2134 Assignment 6}
\author{Lim Wen Bin \\
A0140764H\\
Group 1}
\maketitle

\begin{problem}{1.a.i}
\end{problem}
\begin{proof}
\begin{gather*}
	\frac{\partial \Psi}{\partial t} = \frac{1}{i\hbar}
	\left(-\frac{\hbar^2}{2m} \nabla^2 \Psi + V\Psi \right) \\
	\rho(\mathbf{r},t) = \Psi^*(\mathbf{r}, t) \Psi(\mathbf{r}, t)\\
	\frac{\partial \rho(\mathbf{r},t)}{\partial t} = 
		\Psi^* \frac{\partial \Psi}{\partial t} +
		\frac{\partial \Psi^*}{\partial t} \Psi \\
	-\nabla \cdot \mathbf{j} = 
		\Psi^* \frac{\partial \Psi}{\partial t} +
		\frac{\partial \Psi^*}{\partial t} \Psi \\
	\begin{aligned}
		\nabla \cdot \mathbf{j} &= 
			\frac{\Psi^*}{i\hbar} \left(\frac{\hbar^2}{2m} \nabla^2 \Psi -
			V\Psi \right)
			+ \frac{\Psi}{i\hbar} \left(- \frac{\hbar^2}{2m} \nabla^2 \Psi^* +
			V\Psi^* \right) \\
		&= \frac{\hbar}{2im} ( \Psi^* \nabla^2 \Psi - \Psi \nabla^2 \Psi^*) \\
		&= \frac{\hbar}{2im} ( \Psi^* \nabla \cdot (\nabla \Psi) - \Psi \nabla
			\cdot (\nabla \Psi^*)) \\
		&= \frac{\hbar}{2im} [ \Psi^* \nabla \cdot (\nabla \Psi) 
			+ (\nabla \Psi^*) \cdot (\nabla \Psi)
			- (\nabla \Psi^*) \cdot (\nabla \Psi)
			- \Psi \nabla \cdot (\nabla \Psi^*)]
			\\
		&= \frac{\hbar}{2im} [ \nabla \cdot (\Psi^* (\nabla \Psi))
			- \nabla \cdot (\Psi (\nabla \Psi^*))]
			\\
		&= \frac{\hbar}{2im} \nabla \cdot [ \Psi^* (\nabla \Psi)
			- \Psi (\nabla \Psi^*)]
			\\
		\therefore \mathbf{j} &= 
			\frac{\hbar}{2im} [ \Psi^* (\nabla \Psi)
			- \Psi (\nabla \Psi^*)]
			\\
	\end{aligned}
\end{gather*}
\end{proof}
\filbreak

\begin{problem}{1.a.ii}
\end{problem}
\begin{proof}
Let $\mathcal{R}$ represent the whole space.
\begin{align*}
	\frac{d}{dt} \iiint_{\mathcal{R}} \rho\ dV &= 
		\frac{d}{dt} \iiint_{\mathcal{R}} \Psi^* \Psi \ dV \\
	&= \iiint_{\mathcal{R}} \frac{\partial}{\partial t} (\Psi^* \Psi) \ dV
		\quad (\text{by Leibniz's rule}) \\
	&= \iiint_{\mathcal{R}} \Psi^* \frac{\partial \Psi}{\partial t} +
		\frac{\partial \Psi^*}{\partial t} \Psi \ dV \\
	&= \iiint_{\mathcal{R}} - \nabla \cdot \mathbf{j}
		 \ dV \quad (\text{from (a.i)}) \\
	&= -\iiint_{\mathcal{R}} \frac{\partial j_x}{\partial x}
		+ \frac{\partial j_y}{\partial y}
		+ \frac{\partial j_z}{\partial z}
		\ dV \\
	\iiint_{\mathcal{R}} \frac{\partial j_x}{\partial x} \ dV &=
		\int^\infty_{-\infty} \int^\infty_{-\infty} \int^\infty_{-\infty}
		\frac{\partial j_x}{\partial x} \ dxdydz \\
	&= \int^\infty_{-\infty} \int^\infty_{-\infty} [j_x]^\infty_{-\infty} \
		dydz \\
	&= \int^\infty_{-\infty} \int^\infty_{-\infty}
		 0 \ dydz \quad (\because \Psi \text{ is square integrable}) \\	&= 0
	\intertext{Similarly, $\iiint_{\mathcal{R}} \frac{\partial j_y}{\partial y}
		\ dV = 0$ and $\iiint_{\mathcal{R}} \frac{\partial j_z}{\partial z} \ dV =
		0$. Therefore,}
	\frac{d}{dt} \iiint_{\mathcal{R}} \rho\ dV &= 
		-\iiint_{\mathcal{R}} \frac{\partial j_x}{\partial x}
		+ \frac{\partial j_y}{\partial y}
		+ \frac{\partial j_z}{\partial z}
		\ dV = 0
\end{align*}
\end{proof}
\filbreak

\begin{problem}{1.a.iii}
\end{problem}
\begin{proof}
\begin{align*}
	\intertext{If $V(\mathbf{r}, t)$ is complex,}
		-\frac{\partial \rho}{\partial t} &= 
			\frac{\Psi^*}{i\hbar} \left(\frac{\hbar^2}{2m} \nabla^2 \Psi -
			V\Psi \right)
			+ \frac{\Psi}{i\hbar} \left(- \frac{\hbar^2}{2m} \nabla^2 \Psi^* +
			V^*\Psi^* \right) \\
		&= \nabla \cdot \mathbf{j} + \frac{|\Psi|^2}{i\hbar} (V^* - V) \\
		&= \nabla \cdot \mathbf{j} + \frac{|\Psi|^2}{i\hbar} (-2i\text{Im}[V]) \\
		&= \nabla \cdot \mathbf{j} - \frac{2}{\hbar} \text{Im}[V] \rho \\
	\therefore \frac{\partial \rho}{\partial t} &+ \nabla \cdot \mathbf{j} = 
		\frac{2}{i\hbar} \text{Im}[V] \rho
	\shortintertext{Similarly,}
	\frac{d}{dt} \iiint_{\mathcal{R}} \rho\ dV &= 
		\iiint_{\mathcal{R}} - \nabla \cdot \mathbf{j} \ dV
		+ \iiint_{\mathcal{R}} \frac{2}{\hbar} \text{Im}[V] \rho \ dV \\
	&= \frac{2}{\hbar} \iiint_{\mathcal{R}} \text{Im}[V] \rho \ dV \\
\end{align*}
\end{proof}
\filbreak

\begin{problem}{1.b}
\end{problem}
\begin{align*}
	\frac{\partial \rho}{\partial t} &= - \nabla \cdot \mathbf{j} \\
	&= \nabla \cdot \left[ \frac{i\hbar}{2m} ] \Psi^* (\nabla \Psi)
		- \Psi (\nabla \Psi^*)) \right] \\
	&= \frac{i\hbar}{2m} ( \Psi^* \nabla^2 \Psi
		- \Psi \nabla^2 \Psi^*)
	\intertext{From the Klein-Gordon equation,}
	\nabla^2 \Psi &= \frac{1}{c^2} \frac{\partial^2 \Psi}{\partial t^2} +
		\frac{mc^2}{\hbar^2}\Psi. \\
	\frac{\partial \rho}{\partial t} &=
		\frac{i\hbar}{2m} \left[ \Psi^* \left(
		\frac{1}{c^2} \frac{\partial^2 \Psi}{\partial t^2} +
		\frac{mc^2}{\hbar^2}\Psi
		\right)
		- \Psi  \left(
		\frac{1}{c^2} \frac{\partial^2 \Psi^*}{\partial t^2} +
		\frac{mc^2}{\hbar^2}\Psi^*
		\right) \right] \\
	&= \frac{i\hbar}{2mc^2} \left[ 
		\Psi^* \frac{\partial^2 \Psi}{\partial t^2} 
		- \Psi \frac{\partial^2 \Psi^*}{\partial t^2}
		\right] \\
	&= \frac{i\hbar}{2mc^2} \frac{\partial}{\partial t} \left[ 
		\Psi^* \frac{\partial \Psi}{\partial t} 
		- \Psi \frac{\partial \Psi^*}{\partial t}
		\right] \\
	\therefore \rho &= \frac{i\hbar}{2mc^2} \left[ 
		\Psi^* \frac{\partial \Psi}{\partial t} 
		- \Psi \frac{\partial \Psi^*}{\partial t}
		\right] \\
	\intertext{It would not be appropriate to intepret $\rho$ as the probability
	density as square integrability of the wave function does not imply the
	normalisation of $\rho$.}
\end{align*}

\begin{problem}{2.a}
\end{problem}
\begin{proof}
\begin{gather*}
	\text{Let } \nabla \Phi = \left( \sum_{i=1}^3 \hat{\mathbf{e}}_i' A_i
		\frac{\partial}{\partial u_i} \right) \Phi. \\
	d\Phi = \nabla \Phi \cdot d\mathbf{r} \\
	\sum_{i=1}^3 \frac{\partial \Phi}{\partial u_i} du_i = \left( \sum_{i=1}^3
		\hat{\mathbf{e}}_i' A_i \frac{\partial \Phi}{\partial u_i} \right) \cdot
		\left( \sum_{i=1}^3 h_i du_i \hat{\mathbf{e}}_i' \right) \\
	\Rightarrow A_i = \frac{1}{h_i} \\
	\therefore \nabla \Phi = \left( \sum_{i=1}^3 \hat{\mathbf{e}}_i' \frac{1}{h_i}
		\frac{\partial}{\partial u_i} \right) \Phi. \\
\end{gather*}
\end{proof}
\filbreak

\begin{problem}{2.b}
\end{problem}
\begin{proof}
\begin{gather*}
	\nabla u_i = \sum_{j=1}^3 \hat{\mathbf{e}}_j' \frac{1}{h_j} \frac{\partial
		u_i}{\partial u_j}
		= \sum_{j=1}^3 \hat{\mathbf{e}}_j' \frac{1}{h_j} \delta_{ij} 
		= \hat{\mathbf{e}}_i' \frac{1}{h_i} \\
	\Rightarrow \hat{\mathbf{e}}_i' = h_i \nabla u_i \\
	\begin{aligned}
		\nabla \cdot (a_1 \hat{\mathbf{e}}_1') &= \nabla \cdot [a_1 (\hat{\mathbf{e}}_2'
			\times \hat{\mathbf{e}}_2')] \\
		&= \nabla \cdot [a_1h_2h_3 (\nabla u_2 \times \nabla u_3)] \\
		&= a_1h_2h_3 [\nabla \cdot (\nabla u_2 \times \nabla u_3)] + (\nabla
			a_1h_2h_3) \cdot (\nabla u_2 \times \nabla u_3) \\
		&= a_1h_2h_3 [\nabla u_3 \cdot (\nabla \times \nabla u_2)] + (\nabla
			a_1h_2h_3) \cdot (\nabla u_2 \times \nabla u_3) \\
		&= 0 + (\nabla a_1h_2h_3) \cdot (\nabla u_2 \times \nabla u_3) \\
		&= (\nabla a_1h_2h_3) \cdot \left( \frac{1}{h_2} \hat{\mathbf{e}}_2'
			\times \frac{1}{h_3} \hat{\mathbf{e}}_3' \right) \\
		&= \left[ \left( \sum_{i=1}^3 \hat{\mathbf{e}}_i' \frac{1}{h_i}
			\frac{\partial}{\partial u_i} \right) (a_1h_2h_3) \right] \cdot
			\left( \frac{\hat{\mathbf{e}}_1'}{h_2h_3} \right) \\
		&= \left[ \left( \hat{\mathbf{e}}_1' \frac{1}{h_1}
			\frac{\partial}{\partial u_1} \right) (a_1h_2h_3) \right] \cdot
			\left( \frac{\hat{\mathbf{e}}_1'}{h_2h_3} \right) \\
		&=  \frac{1}{h_1h_2h_3} \frac{\partial}{\partial u_1} \right) (a_1h_2h_3)
	\end{aligned}
	\intertext{Similarly, $\nabla \cdot (a_2 \hat{\mathbf{e}}_2') = 
		\frac{1}{h_1h_2h_3} \frac{\partial}{\partial u_2} \right) (a_2h_1h_3)$
		and $\nabla \cdot (a_3 \hat{\mathbf{e}}_3') = 
		\frac{1}{h_1h_2h_3} \frac{\partial}{\partial u_3} \right) (a_3h_1h_2)$.}
	\therefore \nabla \cdot \mathbf{a} = \sum_{i=1}^3 \nabla \cdot (a_i
		\hat{\mathbf{e}}_i') = \frac{1}{h_1h_2h_3} \left[ 
		\frac{\partial}{\partial u_1} (a_1h_2h_3)
		+ \frac{\partial}{\partial u_2} (a_2h_1h_3)
		+ \frac{\partial}{\partial u_3} (a_3h_1h_2) \right]
\end{gather*}
\end{proof}
\filbreak

\begin{problem}{2.c}
\end{problem}
\begin{proof}
\begin{align*}
	\nabla^2 \Phi &= \nabla \cdot (\nabla \Phi) \\
	&= \nabla \cdot \left( \sum_{i=1}^3 \hat{\mathbf{e}}_i' \frac{1}{h_i}
		\frac{\partial \Phi}{\partial u_i} \right) \\
	&= \frac{1}{h_1h_2h_3} \left[
		\frac{\partial}{\partial u_1} \left( \frac{h_2h_3}{h_1} \frac{\partial
		\Phi}{\partial u_1} \right)
		+ \frac{\partial}{\partial u_2} \left( \frac{h_1h_3}{h_2} \frac{\partial
		\Phi}{\partial u_2} \right)
		+ \frac{\partial}{\partial u_3} \left( \frac{h_1h_2}{h_3} \frac{\partial
		\Phi}{\partial u_3} \right) \right]
\end{align*}
\end{proof}
\filbreak

\begin{problem}{2.d}
\end{problem}
\begin{proof}
\begin{align*}
	\nabla \times (a_1 \hat{\mathbf{e}}_1) &= \nabla \times (a_1 h_1 \nabla u_1) \\
	&= \nabla \times (a_1 h_1 \nabla u_1) \\
	&= (\nabla a_1 h_1) \times (\nabla u_1) 
		+ a_1 h_1 \cdot [\nabla \times (\nabla u_1)] \\
	&= (\nabla a_1 h_1) \times \frac{\hat{\mathbf{e}}_1'}{h_1} + 0 \\
	&= \left( 
			\hat{\mathbf{e}}_2' \frac{1}{h_2} \frac{\partial(a_1h_1)}{\partial u_2} 
			+ \hat{\mathbf{e}}_3' \frac{1}{h_3} \frac{\partial(a_1h_1)}{\partial u_3} 
		\right) 
		\times \frac{\hat{\mathbf{e}}_1'}{h_1} \\
	&=  - \frac{1}{h_1h_2} \frac{\partial(a_1h_1)}{\partial u_2} \hat{\mathbf{e}}_3'
		+ \frac{1}{h_1h_3} \frac{\partial(a_1h_1)}{\partial u_3} \hat{\mathbf{e}}_2' \\
	&=  - \frac{1}{h_1h_2h_3} \frac{\partial(a_1h_1)}{\partial u_2}
		\hat{\mathbf{e}}_3'h_3
		+ \frac{1}{h_1h_2h_3} \frac{\partial(a_1h_1)}{\partial u_3}
		\hat{\mathbf{e}}_2'h_2 
	\shortintertext{Similarly,}
	\nabla \times (a_2 \hat{\mathbf{e}}_2) &= \left( 
			\hat{\mathbf{e}}_1' \frac{1}{h_1} \frac{\partial(a_2h_2)}{\partial u_1} 
			+ \hat{\mathbf{e}}_3' \frac{1}{h_3} \frac{\partial(a_2h_2)}{\partial u_3} 
		\right) 
		\times \frac{\hat{\mathbf{e}}_2'}{h_2} \\
	&=  \frac{1}{h_1h_2h_3} \frac{\partial(a_2h_2)}{\partial u_1}
		\hat{\mathbf{e}}_3'h_3
		+ \frac{1}{h_1h_2h_3} \frac{\partial(a_2h_2)}{\partial u_3}
		\hat{\mathbf{e}}_1'h_1 \\
	\nabla \times (a_3 \hat{\mathbf{e}}_3) &= \left( 
			\hat{\mathbf{e}}_1' \frac{1}{h_1} \frac{\partial(a_3h_3)}{\partial u_1} 
			+ \hat{\mathbf{e}}_2' \frac{1}{h_2} \frac{\partial(a_3h_3)}{\partial u_2} 
		\right) 
		\times \frac{\hat{\mathbf{e}}_3'}{h_3} \\
	&=  - \frac{1}{h_1h_2h_3} \frac{\partial(a_3h_3)}{\partial u_1}
		\hat{\mathbf{e}}_2'h_2
		- \frac{1}{h_1h_2h_3} \frac{\partial(a_3h_3)}{\partial u_2}
		\hat{\mathbf{e}}_1'h_1 \\
	\nabla \times \mathbf{a} &= \sum_{i=1}^3 \nabla \times (a_i \hat{\mathbf{e}}_i)
	\intertext{Rewriting, this yields}
	\nabla \times \mathbf{a} &= \frac{1}{h_1h_2h_3} \left| \begin{array}{ccc}
		\hat{\mathbf{e}}_1'h_1 &
		\hat{\mathbf{e}}_2'h_2 &
		\hat{\mathbf{e}}_3'h_3 \\
		\frac{\partial}{\partial h_1} &
		\frac{\partial}{\partial h_2} &
		\frac{\partial}{\partial h_3} \\
		a_1h_1 &
		a_2h_2 &
		a_3h_3 \\
	\end{array} \right|
\end{align*}
\end{proof}
\filbreak

\begin{problem}{2.e.i}
\end{problem}
\begin{align*}
	\frac{\partial \mathbf{r}}{\partial u} &= \frac{\partial}{\partial u}
		[ (uv\cos\phi) \hat{\mathbf{e}}_x + (uv\sin\phi) \hat{\mathbf{e}}_y
		+ (\frac{1}{2}(u^2 - v^2)) \hat{\mathbf{e}}_z ] \\
	&= (v\cos\phi) \hat{\mathbf{e}}_x + (v\sin\phi) \hat{\mathbf{e}}_y
		+ (u) \hat{\mathbf{e}}_z \\
	\left| \frac{\partial \mathbf{r}}{\partial u} \right| &= \sqrt{u^2 + v^2} \\
	\hat{\mathbf{e}}_u &= \frac{1}{\sqrt{u^2 + v^2}} [ (v\cos\phi)
		\hat{\mathbf{e}}_x + (v\sin\phi) \hat{\mathbf{e}}_y + (u)
		\hat{\mathbf{e}}_z ] \\
	\frac{\partial \mathbf{r}}{\partial v} &= \frac{\partial}{\partial v}
		[ (uv\cos\phi) \hat{\mathbf{e}}_x + (uv\sin\phi) \hat{\mathbf{e}}_y
		+ (\frac{1}{2}(u^2 - v^2)) \hat{\mathbf{e}}_z ] \\
	&= (u\cos\phi) \hat{\mathbf{e}}_x + (u\sin\phi) \hat{\mathbf{e}}_y
		- (v) \hat{\mathbf{e}}_z \\
	\left| \frac{\partial \mathbf{r}}{\partial v} \right| &= \sqrt{u^2 + v^2} \\
	\hat{\mathbf{e}}_v &= \frac{1}{\sqrt{u^2 + v^2}} [ (u\cos\phi)
		\hat{\mathbf{e}}_x + (u\sin\phi) \hat{\mathbf{e}}_y - (v)
		\hat{\mathbf{e}}_z ] \\
	\frac{\partial \mathbf{r}}{\partial \phi} &= \frac{\partial}{\partial \phi}
		[ (uv\cos\phi) \hat{\mathbf{e}}_x + (uv\sin\phi) \hat{\mathbf{e}}_y
		+ (\frac{1}{2}(u^2 - v^2)) \hat{\mathbf{e}}_z ] \\
	&= -(uv\sin\phi) \hat{\mathbf{e}}_x + (uv\cos\phi) \hat{\mathbf{e}}_y \\
	\left| \frac{\partial \mathbf{r}}{\partial \phi} \right| &= uv \\
	\hat{\mathbf{e}}_\phi &= -(\sin\phi) \hat{\mathbf{e}}_x + (\cos\phi)
		\hat{\mathbf{e}}_y \\
	\hat{\mathbf{e}}_u \cdot \hat{\mathbf{e}}_v &= \frac{1}{u^2 + v^2}
		(uv\cos^2\phi + uv\sin^2\phi - uv) = 0 \\
	\hat{\mathbf{e}}_u \cdot \hat{\mathbf{e}}_\phi &= \frac{1}{\sqrt{u^2 +
		v^2}} (-v\cos\phi\sin\phi + v\sin\phi\cos\phi) = 0 \\
	\hat{\mathbf{e}}_v \cdot \hat{\mathbf{e}}_\phi &= \frac{1}{\sqrt{u^2 +
		v^2}} (-u\cos\phi\sin\phi + u\sin\phi\cos\phi) = 0 \\
	\intertext{$\therefore$ The coordinate system is orthogonal.}
	\hat{\mathbf{e}}_u \times \hat{\mathbf{e}}_v &= \frac{1}{u^2 + v^2}
		(-(v^2+u^2)\sin\phi\ \hat{\mathbf{e}}_x + (u^2 + v^2)\cos\phi\
		\hat{\mathbf{e}}_y \\
	&\phantom{=} + (uv\cos\phi\sin\phi - uv\sin\phi\cos\phi)
		\hat{\mathbf{e}}_z = \hat{\mathbf{e}}_\phi \\
	\hat{\mathbf{e}}_\phi \times \hat{\mathbf{e}}_u &= \frac{1}{\sqrt{u^2 + v^2}}
		(u\cos\phi\ \hat{\mathbf{e}}_x + u\sin\phi\ \hat{\mathbf{e}}_y
		- (v\sin^2\phi + v\cos^2\phi) \hat{\mathbf{e}}_z = \hat{\mathbf{e}}_v \\
	\hat{\mathbf{e}}_v \times \hat{\mathbf{e}}_\phi &= \frac{1}{\sqrt{u^2 + v^2}}
		(v\cos\phi\ \hat{\mathbf{e}}_x + v\sin\phi\ \hat{\mathbf{e}}_y
		+ (u\sin^2\phi + u\cos^2\phi) \hat{\mathbf{e}}_z = \hat{\mathbf{e}}_u \\
	\intertext{$\therefore$ The coordinate system is right-handed.}
\end{align*}
\filbreak

\begin{problem}{2.e.ii}
\end{problem}
\begin{gather*}
	\shortintertext{From (i),}
	h_u = \left| \frac{\partial \mathbf{r}}{\partial u} \right| = \sqrt{u^2 + v^2},\
	h_v =\left| \frac{\partial \mathbf{r}}{\partial v} \right| = \sqrt{u^2 + v^2},\
	h_\phi =\left| \frac{\partial \mathbf{r}}{\partial \phi} \right| = uv \\
\end{gather*}
\filbreak

\begin{problem}{2.e.iii}
\end{problem}
\begin{align*}
	[\nabla \times \mathbf{a}]_u &= \frac{1}{h_vh_\phi} \left( \frac{\partial
		(a_\phi h_\phi)} {\partial v} - \frac{\partial (a_vh_v)}{\partial \phi}
		\right) \\
	&= \frac{1}{h_vh_\phi} \left( \frac{\partial (uva_\phi)} {\partial v}
		- \frac{\partial (\sqrt{u^2+v^2}a_v)}{\partial \phi} \right) \\
	&= \frac{1}{uv\sqrt{u^2+v^2}} \left( ua_\phi + uv\frac{\partial a_\phi}
		{\partial v} - \sqrt{u^2+v^2} \frac{\partial a_v}{\partial \phi} \right) \\
	&= \frac{a^3}{v\sqrt{u^2+v^2}} + \frac{1}{\sqrt{u^2+v^2}} \frac{\partial
		a_\phi} {\partial v} - \frac{1}{uv} \frac{\partial a_v}{\partial \phi} \\
\end{align*}
\filbreak

\end{document}
