\documentclass[12pt]{article}
\usepackage[margin=1in]{geometry} 
\usepackage{mathtools,amsmath,amsthm,amssymb,amsfonts}

\newcommand*\diff{\mathop{}\!\mathrm{d}}
\newcommand*\Diff[1]{\mathop{}\!\mathrm{d^#1}} 
\newcommand{\N}{\mathbb{N}}
\newcommand{\Z}{\mathbb{Z}}
 
\newenvironment{problem}[2][Problem]{\begin{trivlist}
\item[\hskip \labelsep {\bfseries #1}\hskip \labelsep {\bfseries #2.}]}{\end{trivlist}}
 
\begin{document}

\title{PC2134 Assignment 7}
\author{Lim Wen Bin \\
A0140764H\\
Group 1}
\maketitle

\begin{problem}{1.a}
\end{problem}
\begin{align*}
	\text{Let } h(x) &= \begin{cases}
		x - 8k, & 0 + 8k \le x < 4 + 8k \\
		-x + 8k, & -4 + 8k \le x < 0 + 8k \\
	\end{cases}, \text{ for $k \in \Z$} \\
	\intertext{As $h(x)$ is even,}
	h(x) &= \frac{a_0}{2} + \sum_{n=1}^\infty a_n \cos \left( \frac{n\pi x}{4} \right) \\
	a_n &= \frac{1}{2} \int_0^4 \cos \left( \frac{n\pi x}{4} \right) x \diff x \\ 
	2a_n &= \frac{4}{n\pi} \left[ \sin \left( \frac{n\pi x}{4} \right) x
		\right]_0^4 - \frac{4}{n\pi} \int_0^4 \sin \left( \frac{n\pi x}{4} \right) 
		\diff x \quad (\text{for } n \ne 0) \\ 
	a_n &= \frac{2}{n\pi} \left[ \sin \left( \frac{n\pi x}{4} \right) x
		\right]_0^4 - \frac{2}{n\pi} \int_0^4 \sin \left( \frac{n\pi x}{4} \right) 
		\diff x \\ 
	&= \frac{8}{n\pi} (\sin (n\pi)) + \frac{8}{(n\pi)^2}
		\left[ \cos \left( \frac{n\pi x}{4} \right) \right]_0^4 \\ 
	&= \frac{8}{(n\pi)^2} \left[ \cos (n\pi) - 1 \right] \\ 
	&= \frac{8}{(n\pi)^2} [(-1)^n - 1] \\ 
	&= \frac{8(-1)^n - 8}{(n\pi)^2} \\ 
	a_0 &= \frac{1}{2} \int_0^4 x \diff x = 4 \\
	\therefore h(x) &= 2 + \sum_{n=1}^\infty \frac{8(-1)^n - 8}{(n\pi)^2} \cos \left(
		\frac{n\pi x}{4} \right) \\
\end{align*}
\begin{align*}
	\intertext{To evaluate $\sum_{n=1}^\infty \frac{(-1)^{n-1}}{n^2}$,}
	h(0) &= 2 + \sum_{n=1}^\infty \frac{8(-1)^n - 8}{(n\pi)^2} = 0. \\
	-2 \left( \frac{\pi^2}{8} \right) &= \sum_{n=1}^\infty \frac{(-1)^n -
		1}{n^2} \\
	\frac{\pi^2}{4} &= \sum_{n=1}^\infty \frac{1 - (-1)^{n-1}}{n^2} \\
	\sum_{n=1}^\infty \frac{(-1)^{n-1}}{n^2} &= \frac{\pi^2}{4}
		-\sum_{n=1}^\infty \frac{1}{n^2} \\
	&= \frac{\pi^2}{4} - \frac{\pi^2}{6} \\
	&= \frac{\pi^2}{12}
	\intertext{To find a Fourier series for $g(x) = x^2$, consider the integral}
	\frac{x^2}{2} &= 2x + \sum_{n=1}^\infty \frac{8(4)}{\pi^3} \left( \frac{(-1)^n
		- 1}{n^3} \right) \sin \left( \frac{n\pi x}{4} \right) + C \\
	g(x) &= 4x + \sum_{n=1}^\infty \frac{64}{\pi^3} \left( \frac{(-1)^n
		- 1}{n^3} \right) \sin \left( \frac{n\pi x}{4} \right) + C \\
\end{align*}
When $x=0$,
\begin{gather*}
	g(0) = 0 + C = 0 \\
	\therefore g(x) = 8 + \sum_{n=1}^\infty \frac{32}{pi^2} \left( \frac{(-1)^n
		- 1}{(n\pi)^2} \right) \cos \left( \frac{n\pi x}{4} \right)
		+ \sum_{n=1}^\infty \frac{64}{\pi^3} \left( \frac{(-1)^n
		- 1}{n^3} \right) \sin \left( \frac{n\pi x}{4} \right)
\end{gather*}
\filbreak

\begin{problem}{1.b}
\end{problem}
\begin{align*}
	\text{Let } l(x) &= \begin{cases}
		x - 8k, & -2 + 8k \le x < 2 + 8k \\
		-x + 8(k+\frac{1}{2}), & 2 + 8k \le x < 6 + 8k \\
	\end{cases}, \text{ for $k \in \Z$} \\
	\intertext{As $g(x)$ is odd,}
	l(x) &= \sum_{n=1}^\infty b_n \sin \left( \frac{n\pi x}{4} \right) \\
	b_n &= \frac{1}{2} \int_0^2 \sin \left( \frac{n\pi x}{4} \right) x \diff x
		+ \frac{1}{2} \int_2^4 \sin \left( \frac{n\pi x}{4} \right) (8-x) \diff x \\
	&=  \int_0^2 \sin \left( \frac{n\pi x}{4} \right) x \diff x \quad
		(\text{by symmetry}) \\ 
	&=  \left[ -\frac{4}{n\pi} \cos \left( \frac{n\pi x}{4} \right) x
		\right]_0^2 + \frac{4}{n\pi} \int_0^2 \cos \left( \frac{n\pi x}{4}
		\right) x \diff x \\
	&=  \frac{4}{n\pi} \int_0^2 \cos \left( \frac{n\pi x}{4} \right) \diff x \\
	&=  \frac{16}{(n\pi)^2} \left[ \sin \left( \frac{n\pi x}{4} \right) \right]_0^2 \\
	&=  \frac{16}{(n\pi)^2} \sin \left( \frac{n\pi}{2} \right) \\
	&=  \begin{cases}
		\frac{16}{(n\pi)^2} (-1)^{(n-1)/2}, & \text{for odd $n$} \\
		0, & \text{for even $n$} \\
		\end{cases} \\
	\therefore l(x) &= \sum_{\substack{n=1,\\ \text{odd $n$}}}^\infty
		\frac{16}{(n\pi)^2} (-1)^{(n-1)/2} \sin \left( \frac{n\pi x}{4} \right) \\
	&= \sum_{n=1}^\infty \frac{16}{\pi^2} \left( \frac{(-1)^{n-1}}{(2n-1)^2}
		\right) \sin \left( \frac{n\pi x}{4} \right) \\
	\intertext{By Parseval's Theorem,}
	\langle [l(x)]^2 \rangle &= \frac{1}{2} \sum_{n=1}^\infty \frac{256}{\pi^4} \left(
		\frac{(-1)^{n-1}}{(2n-1)^2} \right)^2 \\
	&= \frac{128}{\pi^4} \sum_{n=0}^\infty \left( \frac{(-1)^{n}}{(2n+1)^2}
		\right)^2 \\
	&= \frac{128}{\pi^4} \sum_{n=0}^\infty \frac{1}{(2n+1)^4} \\
	\sum_{n=0}^\infty \frac{1}{(2n+1)^4} &= \frac{\pi^4}{128} \left(
		\frac{4}{4} \int_0^2 x^2 \diff x \right) \\
	&= \frac{\pi^4}{256} \left( \frac{8}{3} \right) = \frac{\pi^4}{96}
\end{align*}
\filbreak

\begin{problem}{2}
\end{problem}
The boundary conditions describe a harmonic oscillator system, with an initial
amplitude of 0 and a period of 2. Therefore $x(t)$ is even and can be expressed
as
\begin{align*}
	x(t) &= \sum_{n=1}^\infty b_n \sin (n\pi t). \\
	\ddot{x}(t) &= - \sum_{n=1}^\infty b_n (n\pi)^2 \sin (n\pi t) \\
	\ddot{x} + 4x &= 4t \\
	-(n\pi)^2 b_n + 4 b_n &= 2 \int_0^1 \sin(n\pi t) t \diff t \\
	(4 - (n\pi)^2) b_n &= 2 \int_0^1 \sin(n\pi t) t \diff t \\
	&= \frac{2}{n\pi} \left[ -\cos(n\pi t) t \right]_0^1 + \frac{2}{n\pi}
		\int_0^1 \cos(n\pi t) \diff t \\
	&= -\frac{2}{n\pi} \cos(n\pi) + \frac{2}{(n\pi)^2} \left[ \sin(n\pi t)
		\right]_0^1 \\
	&= \frac{2(-1)^{n-1}}{n\pi} \\
	b_n &= \frac{2(-1)^{n-1}}{(4-(n\pi)^2)n\pi} \\
	\therefore x(t) = \sum_{n=1}^\infty \frac{2(-1)^{n-1}}{(4-(n\pi)^2)n\pi}
		\sin (n\pi t)
\end{align*}

\begin{problem}{3}
\end{problem}
The ratio of the DC output with respect to the incoming input energy can be
found by comparing the mean value of the squares of the respective signals.
\begin{gather*}
	V(x) = \sin(x) \\
	\langle [V(x)]^2 \rangle = \frac{1}{2} 1^2 = \frac{1}{2}
\end{gather*}
To find the Fourier series representation for the rectified signal, $W(x)$,
\begin{align*}
	W(x) &= \frac{a_0}{2} + \sum_{n=1}^\infty a_n \cos(nx) + \sum_{n=1}^\infty
		b_n \sin(nx) \\
	a_n &= \frac{1}{\pi} \int_{-\pi}^\pi \cos (nx) W(x) \diff x \\
	&= \frac{1}{\pi} \int_0^\pi \cos (nx) \sin x \diff x \\
	&= \frac{1}{2\pi} \int_0^\pi \sin ((1-n)x) + \sin((1+n)x) \diff x \\
	&= \frac{1}{2\pi} \left[ \frac{1}{n-1} \cos ((1-n)x) - \frac{1}{n+1}
		\cos((1+n)x) \right]_0^\pi \quad (n \ne 1) \\
	&= \frac{1}{2(n^2-1)\pi} [ (n+1) [(-1)^n - 1] - (n-1) [(-1)^n - 1] ] \\
	&= \frac{(-1)^{n-1} - 1}{(n^2-1)\pi} \\
\begin{align*}
\end{align*}
	a_1 &= \frac{1}{\pi} \int_0^\pi \cos x \sin x \diff x = 0 \\
	%
	b_n &= \frac{1}{\pi} \int_0^\pi \sin (nx) \sin x \diff x \\
	&= \frac{1}{2\pi} \int_0^\pi \cos ((1-n)x) + \cos((1+n)x) \diff x \\
	&= \frac{1}{2\pi} \left[ \frac{1}{1-n} \sin ((1-n)x) - \frac{1}{1+n}
		\sin((1+n)x) \right]_0^\pi \quad (n \ne 1) \\
	&= 0 \\
	b_1 &= \frac{1}{\pi} \int_0^\pi \sin x \sin x \diff x = \frac{1}{2} \\
	\frac{a_0}{2} &= \frac{1}{2} \left( \frac{2}{\pi} \right) = \frac{1}{\pi} \\
	\therefore W(x) &= \frac{1}{\pi} + \frac{1}{2}\sin x + \sum_{n=2}^\infty
		\frac{(-1)^{n-1} - 1}{(n^2-1)\pi} \cos(nx) \\
	&= \frac{1}{\pi} + \frac{1}{2}\sin x + \sum_{n=1}^\infty
		\frac{2}{(1-4n^2)\pi} \cos(2nx) \\
	\langle [W(X)]^2 \rangle &= \frac{1}{\pi^2} + \frac{1}{8} +
		\frac{1}{2}\sum_{n=1}^\infty \frac{4}{(1-4n^2)^2 \pi^2} = \frac{1}{4} \\
	\text{Ratio} &= \frac{\langle [W(X)]^2 \rangle}{\langle [V(X)]^2 \rangle} =
		\frac{1}{2}
\end{align*}
\filbreak

\end{document}
